ok

coq/theories/erasure_type.v
@@ -1,93 +1,93 @@
 From mathcomp Require Import ssreflect ssrbool eqtype ssrnat seq.
 From Stdlib Require Import ssrfun Classical Utf8.
-Require Export AutosubstSsr ARS dyn_sr.
+Require Export AutosubstSsr ARS program_sr.
 
 Set Implicit Arguments.
 Unset Strict Implicit.
 Unset Printing Implicit Defensive.
 
 Reserved Notation "Γ ; Δ ⊢ m ~ n : A" (at level 50, Δ, m, n, A at next level).
-Inductive era_type : sta_ctx -> dyn_ctx -> term -> term -> term -> Prop :=
-| era_var Γ Δ x s A :
-  dyn_wf Γ Δ ->
-  sta_has Γ x A ->
-  dyn_has Δ x s A ->
+Inductive erasure_type : logical_ctx -> program_ctx -> term -> term -> term -> Prop :=
+| erasure_var Γ Δ x s A :
+  program_wf Γ Δ ->
+  logical_has Γ x A ->
+  program_has Δ x s A ->
   Γ ; Δ ⊢ Var x ~ Var x : A
-| era_lam0 Γ Δ A B m m' s :
+| erasure_lam0 Γ Δ A B m m' s :
   Δ ▷ s ->
   (A :: Γ) ; _: Δ ⊢ m ~ m' : B ->
   Γ ; Δ ⊢ Lam0 A m s ~ Lam0 Box m' s : Pi0 A B s
-| era_lam1 Γ Δ A B m m' s t :
+| erasure_lam1 Γ Δ A B m m' s t :
   Δ ▷ s ->
   (A :: Γ) ; A .{t} Δ ⊢ m ~ m' : B ->
   Γ ; Δ ⊢ Lam1 A m s ~ Lam1 Box m' s : Pi1 A B s
-| era_app0 Γ Δ A B m m' n s :
+| erasure_app0 Γ Δ A B m m' n s :
   Γ ; Δ ⊢ m ~ m' : Pi0 A B s ->
   Γ ⊢ n : A ->
   Γ ; Δ ⊢ App m n ~ App m' Box : B.[n/]
-| era_app1 Γ Δ1 Δ2 Δ A B m m' n n' s :
+| erasure_app1 Γ Δ1 Δ2 Δ A B m m' n n' s :
   Δ1 ∘ Δ2 => Δ ->
   Γ ; Δ1 ⊢ m ~ m' : Pi1 A B s ->
   Γ ; Δ2 ⊢ n ~ n' : A ->
   Γ ; Δ ⊢ App m n ~ App m' n' : B.[n/]
-| era_pair0 Γ Δ A B m m' n t l :
+| erasure_pair0 Γ Δ A B m m' n t l :
   Γ ⊢ Sig0 A B t : Sort t l ->
   Γ ; Δ ⊢ m ~ m' : A ->
   Γ ⊢ n : B.[m/] ->
   Γ ; Δ ⊢ Pair0 m n t ~ Pair0 m' Box t : Sig0 A B t
-| era_pair1 Γ Δ1 Δ2 Δ A B m m' n n' t l :
+| erasure_pair1 Γ Δ1 Δ2 Δ A B m m' n n' t l :
   Δ1 ∘ Δ2 => Δ ->
   Γ ⊢ Sig1 A B t : Sort t l ->
   Γ ; Δ1 ⊢ m ~ m' : A ->
   Γ ; Δ2 ⊢ n ~ n' : B.[m/] ->
   Γ ; Δ ⊢ Pair1 m n t ~ Pair1 m' n' t : Sig1 A B t
-| era_letin0 Γ Δ1 Δ2 Δ A B C m m' n n' s r t l :
+| erasure_letin0 Γ Δ1 Δ2 Δ A B C m m' n n' s r t l :
   Δ1 ∘ Δ2 => Δ ->
   (Sig0 A B t :: Γ) ⊢ C : Sort s l ->
   Γ ; Δ1 ⊢ m ~ m' : Sig0 A B t ->
   (B :: A :: Γ) ; _: A .{r} Δ2 ⊢ n ~ n' : C.[Pair0 (Var 1) (Var 0) t .: ren (+2)] ->
   Γ ; Δ ⊢ LetIn C m n ~ LetIn Box m' n' : C.[m/]
-| era_letin1 Γ Δ1 Δ2 Δ A B C m m' n n' s r1 r2 t l :
+| erasure_letin1 Γ Δ1 Δ2 Δ A B C m m' n n' s r1 r2 t l :
   Δ1 ∘ Δ2 => Δ ->
   (Sig1 A B t :: Γ) ⊢ C : Sort s l ->
   Γ ; Δ1 ⊢ m ~ m' : Sig1 A B t ->
   (B :: A :: Γ) ; B .{r2} A .{r1} Δ2 ⊢ n ~ n' : C.[Pair1 (Var 1) (Var 0) t .: ren (+2)] ->
   Γ ; Δ ⊢ LetIn C m n ~ LetIn Box m' n' : C.[m/]
-| era_tt Γ Δ :
-  dyn_wf Γ Δ ->
+| erasure_tt Γ Δ :
+  program_wf Γ Δ ->
   Δ ▷ U ->
   Γ ; Δ ⊢ TT ~ TT : Bool
-| era_ff Γ Δ :
-  dyn_wf Γ Δ ->
+| erasure_ff Γ Δ :
+  program_wf Γ Δ ->
   Δ ▷ U ->
   Γ ; Δ ⊢ FF ~ FF : Bool
-| era_ifte Γ Δ1 Δ2 Δ A m m' n1 n1' n2 n2' s l :
+| erasure_ifte Γ Δ1 Δ2 Δ A m m' n1 n1' n2 n2' s l :
   Δ1 ∘ Δ2 => Δ ->
   (Bool :: Γ) ⊢ A : Sort s l ->
   Γ ; Δ1 ⊢ m ~ m' : Bool ->
   Γ ; Δ2 ⊢ n1 ~ n1' : A.[TT/] ->
   Γ ; Δ2 ⊢ n2 ~ n2' : A.[FF/] ->
   Γ ; Δ ⊢ Ifte A m n1 n2 ~ Ifte Box m' n1' n2' : A.[m/]
-| era_rw Γ Δ A B H H' P m n s l :
+| erasure_rw Γ Δ A B H H' P m n s l :
   (Id A.[ren (+1)] m.[ren (+1)] (Var 0) :: A :: Γ) ⊢ B : Sort s l ->
   Γ ; Δ ⊢ H ~ H' : B.[Refl m,m/] ->
   Γ ⊢ P : Id A m n ->
   Γ ; Δ ⊢ Rw B H P ~ Rw Box H' Box : B.[P,n/]
-| era_conv Γ Δ A B m m' s l :
+| erasure_conv Γ Δ A B m m' s l :
   A ≃ B ->
   Γ ; Δ ⊢ m ~ m' : A ->
   Γ ⊢ B : Sort s l ->
   Γ ; Δ ⊢ m ~ m' : B
-where "Γ ; Δ ⊢ m ~ n : A" := (era_type Γ Δ m n A).
+where "Γ ; Δ ⊢ m ~ n : A" := (erasure_type Γ Δ m n A).
 
-Lemma era_dyn_type Γ Δ m m' A :
+Lemma erasure_program_type Γ Δ m m' A :
   Γ ; Δ ⊢ m ~ m' : A -> Γ ; Δ ⊢ m : A.
-Proof with eauto using dyn_type. elim... Qed.
-#[global] Hint Resolve era_dyn_type.
+Proof with eauto using program_type. elim... Qed.
+#[global] Hint Resolve erasure_program_type.
 
-Lemma dyn_era_type Γ Δ m A :
+Lemma program_erasure_type Γ Δ m A :
   Γ ; Δ ⊢ m : A -> exists m', Γ ; Δ ⊢ m ~ m' : A.
-Proof with eauto using era_type.
+Proof with eauto using erasure_type.
   elim=>{Γ Δ m A}.
   { move=>Γ Δ x A wf shs dhs. exists (Var x)... }
   { move=>Γ Δ A B m s k tym[m' er].
@@ -112,7 +112,7 @@ Proof with eauto using era_type.
     exists (Ifte Box m' n1' n2')... }
   { move=>Γ Δ A B H P m n s l tyB tyH[H' erH]tyP.
     exists (Rw Box H' Box).
-    apply: era_rw... }
+    apply: erasure_rw... }
   { move=>Γ Δ A B m s l eq tym[m' er]tyB.
-    exists m'. apply: era_conv... }
+    exists m'. apply: erasure_conv... }
 Qed.
