coq/theories/heap_step.v
@@ -1,70 +1,70 @@
 From mathcomp Require Import ssreflect ssrbool eqtype ssrnat seq.
 From Stdlib Require Import ssrfun Classical Utf8.
-Require Export AutosubstSsr ARS ptr_res.
+Require Export AutosubstSsr ARS heap_res.
 
 Set Implicit Arguments.
 Unset Strict Implicit.
 Unset Printing Implicit Defensive.
 
 Reserved Notation "H1 ; m ~>> H2 ; n" (at level 50, m, H2, n at next level).
-Inductive ptr_step : heap -> term -> heap -> term -> Prop :=
-| ptr_step_lam0 H m s l :
+Inductive heap_step : heap -> term -> heap -> term -> Prop :=
+| heap_step_lam0 H m s l :
   l \notin domm H ->
   H ; Lam0 Box m s ~>> setm H l (Lam0 Box m s, s) ; Ptr l
-| ptr_step_lam1 H m s l :
+| heap_step_lam1 H m s l :
   l \notin domm H ->
   H ; Lam1 Box m s ~>> setm H l (Lam1 Box m s, s) ; (Ptr l)
-| ptr_step_appL H H' m m' n :
+| heap_step_appL H H' m m' n :
   H ; m ~>> H' ; m' ->
   H ; App m n ~>> H' ; App m' n
-| ptr_step_appR H H' m n n' :
+| heap_step_appR H H' m n n' :
   H ; n ~>> H' ; n' ->
   H ; App m n ~>> H' ; App m n'
-| ptr_step_beta0 H H' l m n s :
+| heap_step_beta0 H H' l m n s :
   free H l (Lam0 Box m s) H' ->
   H ; App (Ptr l) n ~>> H' ; m.[Box/]
-| ptr_step_beta1 H H' lf la m s :
+| heap_step_beta1 H H' lf la m s :
   free H lf (Lam1 Box m s) H' ->
   H ; App (Ptr lf) (Ptr la) ~>> H' ; m.[Ptr la/]
-| ptr_step_pair0L H H' m m' t :
+| heap_step_pair0L H H' m m' t :
   H ; m ~>> H' ; m' ->
   H ; Pair0 m Box t ~>> H' ; Pair0 m' Box t
-| ptr_step_pair0 H l lm t :
+| heap_step_pair0 H l lm t :
   l \notin domm H ->
   H ; Pair0 (Ptr lm) Box t ~>> setm H l (Pair0 (Ptr lm) Box t, t) ; Ptr l
-| ptr_step_pair1L H H' m m' n t :
+| heap_step_pair1L H H' m m' n t :
   H ; m ~>> H' ; m' ->
   H ; Pair1 m n t ~>> H' ; Pair1 m' n t
-| ptr_step_pair1R H H' m n n' t :
+| heap_step_pair1R H H' m n n' t :
   H ; n ~>> H' ; n' ->
   H ; Pair1 m n t ~>> H' ; Pair1 m n' t
-| ptr_step_pair1 H l lm ln t :
+| heap_step_pair1 H l lm ln t :
   l \notin domm H ->
   H ; Pair1 (Ptr lm) (Ptr ln) t ~>> setm H l (Pair1 (Ptr lm) (Ptr ln) t, t) ; Ptr l
-| ptr_step_letinL H H' m m' n :
+| heap_step_letinL H H' m m' n :
   H ; m ~>> H' ; m' ->
   H ; LetIn Box m n ~>> H' ; LetIn Box m' n
-| ptr_step_iota0 H H' lm x l n t :
+| heap_step_iota0 H H' lm x l n t :
   free H l (Pair0 (Ptr lm) x t) H' ->
   H ; LetIn Box (Ptr l) n ~>> H' ; n.[Box,Ptr lm/]
-| ptr_step_iota1 H H' lm ln l n t :
+| heap_step_iota1 H H' lm ln l n t :
   free H l (Pair1 (Ptr lm) (Ptr ln) t) H' ->
   H ; LetIn Box (Ptr l) n ~>> H' ; n.[Ptr ln,Ptr lm/]
-| ptr_step_tt H l :
+| heap_step_tt H l :
   l \notin domm H ->
   H ; TT ~>> setm H l (TT, U) ; (Ptr l)
-| ptr_step_ff H l :
+| heap_step_ff H l :
   l \notin domm H ->
   H ; FF ~>> setm H l (FF, U) ; (Ptr l)
-| ptr_step_ifteM H H' m m' n1 n2 :
+| heap_step_ifteM H H' m m' n1 n2 :
   H ; m ~>> H' ; m' ->
   H ; Ifte Box m n1 n2 ~>> H' ; Ifte Box m' n1 n2
-| ptr_step_ifteT H H' l n1 n2 :
+| heap_step_ifteT H H' l n1 n2 :
   free H l TT H' ->
   H ; Ifte Box (Ptr l) n1 n2 ~>> H' ; n1
-| ptr_step_ifteF H H' l n1 n2 :
+| heap_step_ifteF H H' l n1 n2 :
   free H l FF H' ->
   H ; Ifte Box (Ptr l) n1 n2 ~>> H' ; n2
-| ptr_step_rwE H m :
+| heap_step_rwE H m :
   H ; Rw Box m Box ~>> H ; m
-where "H1 ; m ~>> H2 ; n" := (ptr_step H1 m H2 n).
+where "H1 ; m ~>> H2 ; n" := (heap_step H1 m H2 n).
