coq/theories/logical_conf.v
@@ -1,6 +1,6 @@
 From mathcomp Require Import ssreflect ssrbool eqtype ssrnat seq.
 From Stdlib Require Import ssrfun Classical Utf8.
-Require Export AutosubstSsr ARS sta_step.
+Require Export AutosubstSsr ARS logical_step.
 
 Set Implicit Arguments.
 Unset Strict Implicit.
@@ -105,175 +105,175 @@ Inductive pstep : term -> term -> Prop :=
   pstep H H' ->
   pstep (Rw A H (Refl m)) H'
 | pstep_box : pstep Box Box
-| pstep_ptr l : pstep (Ptr l) (Ptr l).
+| pstep_heap l : pstep (Ptr l) (Ptr l).
 
 Definition sred σ τ := forall x : var, (σ x) ~>* (τ x).
 
-Lemma sta_step_subst σ m n : m ~> n -> m.[σ] ~> n.[σ].
+Lemma logical_step_subst σ m n : m ~> n -> m.[σ] ~> n.[σ].
 Proof.
-  move=> st. elim: st σ=>/={m n}; eauto using sta_step.
+  move=> st. elim: st σ=>/={m n}; eauto using logical_step.
   { move=> A m n s σ.
     replace (m.[n/].[σ]) with (m.[up σ].[n.[σ]/]).
-    apply sta_step_beta0. autosubst. }
+    apply logical_step_beta0. autosubst. }
   { move=> A m n s σ.
     replace (m.[n/].[σ]) with (m.[up σ].[n.[σ]/]).
-    apply sta_step_beta1. autosubst. }
+    apply logical_step_beta1. autosubst. }
   { move=>A m1 m2 n s σ.
     replace (n.[m2,m1/].[σ]) with (n.[upn 2 σ].[m2.[σ],m1.[σ]/]).
-    apply: sta_step_iota0. autosubst. }
+    apply: logical_step_iota0. autosubst. }
   { move=>A m1 m2 n s σ.
     replace (n.[m2,m1/].[σ]) with (n.[upn 2 σ].[m2.[σ],m1.[σ]/]).
-    apply: sta_step_iota1. autosubst. }
+    apply: logical_step_iota1. autosubst. }
 Qed.
 
-Lemma sta_red_app m m' n n' :
+Lemma logical_red_app m m' n n' :
   m ~>* m' -> n ~>* n' -> App m n ~>* App m' n'.
 Proof.
   move=> r1 r2.
   apply: (star_trans (App m' n)).
-  apply: (star_hom (App^~ n)) r1=>x y. exact: sta_step_appL.
-  apply: star_hom r2. exact: sta_step_appR.
+  apply: (star_hom (App^~ n)) r1=>x y. exact: logical_step_appL.
+  apply: star_hom r2. exact: logical_step_appR.
 Qed.
 
-Lemma sta_red_lam0 A A' m m' s :
+Lemma logical_red_lam0 A A' m m' s :
   A ~>* A' -> m ~>* m' -> Lam0 A m s ~>* Lam0 A' m' s.
 Proof.
   move=> r1 r2.
   apply: (star_trans (Lam0 A' m s)).
-  apply: (star_hom ((Lam0^~ m)^~ s)) r1=>x y. exact: sta_step_lam0L.
-  apply: (star_hom ((Lam0 A')^~ s)) r2=>x y. exact: sta_step_lam0R.
+  apply: (star_hom ((Lam0^~ m)^~ s)) r1=>x y. exact: logical_step_lam0L.
+  apply: (star_hom ((Lam0 A')^~ s)) r2=>x y. exact: logical_step_lam0R.
 Qed.
 
-Lemma sta_red_lam1 A A' m m' s :
+Lemma logical_red_lam1 A A' m m' s :
   A ~>* A' -> m ~>* m' -> Lam1 A m s ~>* Lam1 A' m' s.
 Proof.
   move=> r1 r2.
   apply: (star_trans (Lam1 A' m s)).
-  apply: (star_hom ((Lam1^~ m)^~ s)) r1=>x y. exact: sta_step_lam1L.
-  apply: (star_hom ((Lam1 A')^~ s)) r2=>x y. exact: sta_step_lam1R.
+  apply: (star_hom ((Lam1^~ m)^~ s)) r1=>x y. exact: logical_step_lam1L.
+  apply: (star_hom ((Lam1 A')^~ s)) r2=>x y. exact: logical_step_lam1R.
 Qed.
 
-Lemma sta_red_pi0 A A' B B' s :
+Lemma logical_red_pi0 A A' B B' s :
   A ~>* A' -> B ~>* B' -> Pi0 A B s ~>* Pi0 A' B' s.
 Proof.
   move=> r1 r2.
   apply: (star_trans (Pi0 A' B s)).
-  apply: (star_hom ((Pi0^~ B)^~ s)) r1=>x y. exact: sta_step_pi0L.
-  apply: (star_hom ((Pi0 A')^~ s)) r2=>x y. exact: sta_step_pi0R.
+  apply: (star_hom ((Pi0^~ B)^~ s)) r1=>x y. exact: logical_step_pi0L.
+  apply: (star_hom ((Pi0 A')^~ s)) r2=>x y. exact: logical_step_pi0R.
 Qed.
 
-Lemma sta_red_pi1 A A' B B' s :
+Lemma logical_red_pi1 A A' B B' s :
   A ~>* A' -> B ~>* B' -> Pi1 A B s ~>* Pi1 A' B' s.
 Proof.
   move=> r1 r2.
   apply: (star_trans (Pi1 A' B s)).
-  apply: (star_hom ((Pi1^~ B)^~ s)) r1=>x y. exact: sta_step_pi1L.
-  apply: (star_hom ((Pi1 A')^~ s)) r2=>x y. exact: sta_step_pi1R.
+  apply: (star_hom ((Pi1^~ B)^~ s)) r1=>x y. exact: logical_step_pi1L.
+  apply: (star_hom ((Pi1 A')^~ s)) r2=>x y. exact: logical_step_pi1R.
 Qed.
 
-Lemma sta_red_sig0 A A' B B' s :
+Lemma logical_red_sig0 A A' B B' s :
   A ~>* A' -> B ~>* B' -> Sig0 A B s ~>* Sig0 A' B' s.
 Proof.
   move=> r1 r2.
   apply: (star_trans (Sig0 A' B s)).
-  apply: (star_hom ((Sig0^~ B)^~ s)) r1=>x y. exact: sta_step_sig0L.
-  apply: (star_hom ((Sig0 A')^~ s)) r2=>x y. exact: sta_step_sig0R.
+  apply: (star_hom ((Sig0^~ B)^~ s)) r1=>x y. exact: logical_step_sig0L.
+  apply: (star_hom ((Sig0 A')^~ s)) r2=>x y. exact: logical_step_sig0R.
 Qed.
 
-Lemma sta_red_sig1 A A' B B' s :
+Lemma logical_red_sig1 A A' B B' s :
   A ~>* A' -> B ~>* B' -> Sig1 A B s ~>* Sig1 A' B' s.
 Proof.
   move=> r1 r2.
   apply: (star_trans (Sig1 A' B s)).
-  apply: (star_hom ((Sig1^~ B)^~ s)) r1=>x y. exact: sta_step_sig1L.
-  apply: (star_hom ((Sig1 A')^~ s)) r2=>x y. exact: sta_step_sig1R.
+  apply: (star_hom ((Sig1^~ B)^~ s)) r1=>x y. exact: logical_step_sig1L.
+  apply: (star_hom ((Sig1 A')^~ s)) r2=>x y. exact: logical_step_sig1R.
 Qed.
 
-Lemma sta_red_pair0 m m' n n' t :
+Lemma logical_red_pair0 m m' n n' t :
   m ~>* m' -> n ~>* n' -> Pair0 m n t ~>* Pair0 m' n' t.
 Proof.
   move=>r1 r2.
   apply: (star_trans (Pair0 m' n t)).
-  apply: (star_hom ((Pair0^~ n)^~ t)) r1=>x y. exact: sta_step_pair0L.
-  apply: (star_hom ((Pair0 m')^~ t)) r2=>x y. exact: sta_step_pair0R.
+  apply: (star_hom ((Pair0^~ n)^~ t)) r1=>x y. exact: logical_step_pair0L.
+  apply: (star_hom ((Pair0 m')^~ t)) r2=>x y. exact: logical_step_pair0R.
 Qed.
 
-Lemma sta_red_pair1 m m' n n' t :
+Lemma logical_red_pair1 m m' n n' t :
   m ~>* m' -> n ~>* n' -> Pair1 m n t ~>* Pair1 m' n' t.
 Proof.
   move=>r1 r2.
   apply: (star_trans (Pair1 m' n t)).
-  apply: (star_hom ((Pair1^~ n)^~ t)) r1=>x y. exact: sta_step_pair1L.
-  apply: (star_hom ((Pair1 m')^~ t)) r2=>x y. exact: sta_step_pair1R.
+  apply: (star_hom ((Pair1^~ n)^~ t)) r1=>x y. exact: logical_step_pair1L.
+  apply: (star_hom ((Pair1 m')^~ t)) r2=>x y. exact: logical_step_pair1R.
 Qed.
 
-Lemma sta_red_letin A A' m m' n n' :
+Lemma logical_red_letin A A' m m' n n' :
   A ~>* A' -> m ~>* m' -> n ~>* n' -> LetIn A m n ~>* LetIn A' m' n'.
 Proof.
   move=>r1 r2 r3.
   apply: (star_trans (LetIn A' m n)).
-  apply: (star_hom ((LetIn^~ m)^~ n)) r1=>x y. exact: sta_step_letinA.
+  apply: (star_hom ((LetIn^~ m)^~ n)) r1=>x y. exact: logical_step_letinA.
   apply: (star_trans (LetIn A' m' n)).
-  apply: (star_hom (LetIn A'^~ n)) r2=>x y. exact: sta_step_letinL.
-  apply: (star_hom (LetIn A' m')) r3=>x y. exact: sta_step_letinR.
+  apply: (star_hom (LetIn A'^~ n)) r2=>x y. exact: logical_step_letinL.
+  apply: (star_hom (LetIn A' m')) r3=>x y. exact: logical_step_letinR.
 Qed.
 
-Lemma sta_red_ifte A A' m m' n1 n1' n2 n2' :
+Lemma logical_red_ifte A A' m m' n1 n1' n2 n2' :
   A ~>* A' -> m ~>* m' -> n1 ~>* n1' -> n2 ~>* n2' -> Ifte A m n1 n2 ~>* Ifte A' m' n1' n2'.
 Proof.
   move=>rA rm rn1 rn2.
   apply: (star_trans (Ifte A' m n1 n2)).
-  apply: (star_hom (((Ifte^~ m)^~ n1)^~ n2)) rA=>x y. exact: sta_step_ifteA.
+  apply: (star_hom (((Ifte^~ m)^~ n1)^~ n2)) rA=>x y. exact: logical_step_ifteA.
   apply: (star_trans (Ifte A' m' n1 n2)).
-  apply: (star_hom (((Ifte A')^~ n1)^~ n2)) rm=>x y. exact: sta_step_ifteM.
+  apply: (star_hom (((Ifte A')^~ n1)^~ n2)) rm=>x y. exact: logical_step_ifteM.
   apply: (star_trans (Ifte A' m' n1' n2)).
-  apply: (star_hom ((Ifte A' m')^~ n2)) rn1=>x y. exact: sta_step_ifteN1.
-  apply: (star_hom (Ifte A' m' n1')) rn2=>x y. exact: sta_step_ifteN2.
+  apply: (star_hom ((Ifte A' m')^~ n2)) rn1=>x y. exact: logical_step_ifteN1.
+  apply: (star_hom (Ifte A' m' n1')) rn2=>x y. exact: logical_step_ifteN2.
 Qed.
 
-Lemma sta_red_id A A' m m' n n' :
+Lemma logical_red_id A A' m m' n n' :
   A ~>* A' -> m ~>* m' -> n ~>* n' -> Id A m n ~>* Id A' m' n'.
 Proof.
   move=>r1 r2 r3.
   apply: (star_trans (Id A' m n)).
-  apply: (star_hom ((Id^~ m)^~ n)) r1=>x y. exact: sta_step_idA.
+  apply: (star_hom ((Id^~ m)^~ n)) r1=>x y. exact: logical_step_idA.
   apply: (star_trans (Id A' m' n)).
-  apply: (star_hom (Id A'^~ n)) r2=>x y. exact: sta_step_idL.
-  apply: (star_hom (Id A' m')) r3=>x y. exact: sta_step_idR.
+  apply: (star_hom (Id A'^~ n)) r2=>x y. exact: logical_step_idL.
+  apply: (star_hom (Id A' m')) r3=>x y. exact: logical_step_idR.
 Qed.
 
-Lemma sta_red_refl m m' :
+Lemma logical_red_refl m m' :
   m ~>* m' -> Refl m ~>* Refl m'.
 Proof.
   move=>r.
-  apply: (star_hom Refl) r=>x y. exact: sta_step_refl.
+  apply: (star_hom Refl) r=>x y. exact: logical_step_refl.
 Qed.
 
-Lemma sta_red_rw A A' H H' P P' :
+Lemma logical_red_rw A A' H H' P P' :
   A ~>* A' -> H ~>* H' -> P ~>* P' -> Rw A H P ~>* Rw A' H' P'.
 Proof.
   move=>r1 r2 r3.
   apply: (star_trans (Rw A' H P)).
-  apply: (star_hom ((Rw^~ H)^~ P)) r1=>x y. exact: sta_step_rwA.
+  apply: (star_hom ((Rw^~ H)^~ P)) r1=>x y. exact: logical_step_rwA.
   apply: (star_trans (Rw A' H' P)).
-  apply: (star_hom (Rw A'^~P)) r2=>x y. exact: sta_step_rwH.
-  apply: (star_hom (Rw A' H')) r3=>x y. exact: sta_step_rwP.
+  apply: (star_hom (Rw A'^~P)) r2=>x y. exact: logical_step_rwH.
+  apply: (star_hom (Rw A' H')) r3=>x y. exact: logical_step_rwP.
 Qed.
 
-Lemma sta_red_subst m n σ : m ~>* n -> m.[σ] ~>* n.[σ].
+Lemma logical_red_subst m n σ : m ~>* n -> m.[σ] ~>* n.[σ].
 Proof.
   move=>st.
   elim: st σ=>{n}; eauto.
   move=> n n' r ih st σ.
   move:(ih σ)=>{}ih.
-  move:(sta_step_subst σ st)=>r'.
+  move:(logical_step_subst σ st)=>r'.
   apply: star_trans.
   apply: ih.
   by apply: star1.
 Qed.
 
 Lemma sred_up σ τ : sred σ τ -> sred (up σ) (up τ).
-Proof. move=> A [|n] //=. asimpl. apply: sta_red_subst. exact: A. Qed.
+Proof. move=> A [|n] //=. asimpl. apply: logical_red_subst. exact: A. Qed.
 
 Lemma sred_upn n σ τ : sred σ τ -> sred (upn n σ) (upn n τ).
 Proof.
@@ -283,164 +283,164 @@ Proof.
 Qed.
 
 #[global] Hint Resolve
-  sta_red_app
-  sta_red_lam0 sta_red_lam1
-  sta_red_pi0 sta_red_pi1
-  sta_red_sig0 sta_red_sig1
-  sta_red_pair0 sta_red_pair1
-  sta_red_letin sta_red_ifte
-  sta_red_id sta_red_refl sta_red_rw
-  sred_up sred_upn : sta_red_congr.
+  logical_red_app
+  logical_red_lam0 logical_red_lam1
+  logical_red_pi0 logical_red_pi1
+  logical_red_sig0 logical_red_sig1
+  logical_red_pair0 logical_red_pair1
+  logical_red_letin logical_red_ifte
+  logical_red_id logical_red_refl logical_red_rw
+  sred_up sred_upn : logical_red_congr.
 
-Lemma sta_red_compat σ τ s : sred σ τ -> sta_red s.[σ] s.[τ].
-Proof. elim: s σ τ => *; asimpl; eauto 9 with sta_red_congr. Qed.
+Lemma logical_red_compat σ τ s : sred σ τ -> logical_red s.[σ] s.[τ].
+Proof. elim: s σ τ => *; asimpl; eauto 9 with logical_red_congr. Qed.
 
 Definition sconv (σ τ : var -> term) := forall x, σ x ≃ τ x.
 
-Lemma sta_conv_app m m' n n' :
+Lemma logical_conv_app m m' n n' :
   m ≃ m' -> n ≃ n' -> App m n ≃ App m' n'.
 Proof.
   move=> r1 r2.
   apply: (conv_trans (App m' n)).
-  apply: (conv_hom (App^~ n)) r1=>x y. exact: sta_step_appL.
-  apply: conv_hom r2. exact: sta_step_appR.
+  apply: (conv_hom (App^~ n)) r1=>x y. exact: logical_step_appL.
+  apply: conv_hom r2. exact: logical_step_appR.
 Qed.
 
-Lemma sta_conv_lam0 A A' m m' s :
+Lemma logical_conv_lam0 A A' m m' s :
   A ≃ A' -> m ≃ m' -> Lam0 A m s ≃ Lam0 A' m' s.
 Proof.
   move=> r1 r2.
   apply: (conv_trans (Lam0 A' m s)).
-  apply: (conv_hom ((Lam0^~ m)^~ s)) r1=>x y. exact: sta_step_lam0L.
-  apply: (conv_hom ((Lam0 A')^~ s)) r2=>x y. exact: sta_step_lam0R.
+  apply: (conv_hom ((Lam0^~ m)^~ s)) r1=>x y. exact: logical_step_lam0L.
+  apply: (conv_hom ((Lam0 A')^~ s)) r2=>x y. exact: logical_step_lam0R.
 Qed.
 
-Lemma sta_conv_lam1 A A' m m' s :
+Lemma logical_conv_lam1 A A' m m' s :
   A ≃ A' -> m ≃ m' -> Lam1 A m s ≃ Lam1 A' m' s.
 Proof.
   move=> r1 r2.
   apply: (conv_trans (Lam1 A' m s)).
-  apply: (conv_hom ((Lam1^~ m)^~ s)) r1=>x y. exact: sta_step_lam1L.
-  apply: (conv_hom ((Lam1 A')^~ s)) r2=>x y. exact: sta_step_lam1R.
+  apply: (conv_hom ((Lam1^~ m)^~ s)) r1=>x y. exact: logical_step_lam1L.
+  apply: (conv_hom ((Lam1 A')^~ s)) r2=>x y. exact: logical_step_lam1R.
 Qed.
 
-Lemma sta_conv_pi0 A A' B B' s :
+Lemma logical_conv_pi0 A A' B B' s :
   A ≃ A' -> B ≃ B' -> Pi0 A B s ≃ Pi0 A' B' s.
 Proof.
   move=> r1 r2.
   apply: (conv_trans (Pi0 A' B s)).
-  apply: (conv_hom ((Pi0^~ B)^~ s)) r1=>x y. exact: sta_step_pi0L.
-  apply: (conv_hom ((Pi0 A')^~ s)) r2=>x y. exact: sta_step_pi0R.
+  apply: (conv_hom ((Pi0^~ B)^~ s)) r1=>x y. exact: logical_step_pi0L.
+  apply: (conv_hom ((Pi0 A')^~ s)) r2=>x y. exact: logical_step_pi0R.
 Qed.
 
-Lemma sta_conv_pi1 A A' B B' s :
+Lemma logical_conv_pi1 A A' B B' s :
   A ≃ A' -> B ≃ B' -> Pi1 A B s ≃ Pi1 A' B' s.
 Proof.
   move=> r1 r2.
   apply: (conv_trans (Pi1 A' B s)).
-  apply: (conv_hom ((Pi1^~ B)^~ s)) r1=>x y. exact: sta_step_pi1L.
-  apply: (conv_hom ((Pi1 A')^~ s)) r2=>x y. exact: sta_step_pi1R.
+  apply: (conv_hom ((Pi1^~ B)^~ s)) r1=>x y. exact: logical_step_pi1L.
+  apply: (conv_hom ((Pi1 A')^~ s)) r2=>x y. exact: logical_step_pi1R.
 Qed.
 
-Lemma sta_conv_sig0 A A' B B' s :
+Lemma logical_conv_sig0 A A' B B' s :
   A ≃ A' -> B ≃ B' -> Sig0 A B s ≃ Sig0 A' B' s.
 Proof.
   move=> r1 r2.
   apply: (conv_trans (Sig0 A' B s)).
-  apply: (conv_hom ((Sig0^~ B)^~ s)) r1=>x y. exact: sta_step_sig0L.
-  apply: (conv_hom ((Sig0 A')^~ s)) r2=>x y. exact: sta_step_sig0R.
+  apply: (conv_hom ((Sig0^~ B)^~ s)) r1=>x y. exact: logical_step_sig0L.
+  apply: (conv_hom ((Sig0 A')^~ s)) r2=>x y. exact: logical_step_sig0R.
 Qed.
 
-Lemma sta_conv_sig1 A A' B B' s :
+Lemma logical_conv_sig1 A A' B B' s :
   A ≃ A' -> B ≃ B' -> Sig1 A B s ≃ Sig1 A' B' s.
 Proof.
   move=> r1 r2.
   apply: (conv_trans (Sig1 A' B s)).
-  apply: (conv_hom ((Sig1^~ B)^~ s)) r1=>x y. exact: sta_step_sig1L.
-  apply: (conv_hom ((Sig1 A')^~ s)) r2=>x y. exact: sta_step_sig1R.
+  apply: (conv_hom ((Sig1^~ B)^~ s)) r1=>x y. exact: logical_step_sig1L.
+  apply: (conv_hom ((Sig1 A')^~ s)) r2=>x y. exact: logical_step_sig1R.
 Qed.
 
-Lemma sta_conv_pair0 m m' n n' t :
+Lemma logical_conv_pair0 m m' n n' t :
   m ≃ m' -> n ≃ n' -> Pair0 m n t ≃ Pair0 m' n' t.
 Proof.
   move=>r1 r2.
   apply: (conv_trans (Pair0 m' n t)).
-  apply: (conv_hom ((Pair0^~ n)^~ t)) r1=>x y. exact: sta_step_pair0L.
-  apply: (conv_hom ((Pair0 m')^~ t)) r2=>x y. exact: sta_step_pair0R.
+  apply: (conv_hom ((Pair0^~ n)^~ t)) r1=>x y. exact: logical_step_pair0L.
+  apply: (conv_hom ((Pair0 m')^~ t)) r2=>x y. exact: logical_step_pair0R.
 Qed.
 
-Lemma sta_conv_pair1 m m' n n' t :
+Lemma logical_conv_pair1 m m' n n' t :
   m ≃ m' -> n ≃ n' -> Pair1 m n t ≃ Pair1 m' n' t.
 Proof.
   move=>r1 r2.
   apply: (conv_trans (Pair1 m' n t)).
-  apply: (conv_hom ((Pair1^~ n)^~ t)) r1=>x y. exact: sta_step_pair1L.
-  apply: (conv_hom ((Pair1 m')^~ t)) r2=>x y. exact: sta_step_pair1R.
+  apply: (conv_hom ((Pair1^~ n)^~ t)) r1=>x y. exact: logical_step_pair1L.
+  apply: (conv_hom ((Pair1 m')^~ t)) r2=>x y. exact: logical_step_pair1R.
 Qed.
 
-Lemma sta_conv_letin A A' m m' n n' :
+Lemma logical_conv_letin A A' m m' n n' :
   A ≃ A' -> m ≃ m' -> n ≃ n' -> LetIn A m n ≃ LetIn A' m' n'.
 Proof.
   move=>r1 r2 r3.
   apply: (conv_trans (LetIn A' m n)).
-  apply: (conv_hom ((LetIn^~ m)^~ n)) r1=>x y. exact: sta_step_letinA.
+  apply: (conv_hom ((LetIn^~ m)^~ n)) r1=>x y. exact: logical_step_letinA.
   apply: (conv_trans (LetIn A' m' n)).
-  apply: (conv_hom (LetIn A'^~ n)) r2=>x y. exact: sta_step_letinL.
-  apply: (conv_hom (LetIn A' m')) r3=>x y. exact: sta_step_letinR.
+  apply: (conv_hom (LetIn A'^~ n)) r2=>x y. exact: logical_step_letinL.
+  apply: (conv_hom (LetIn A' m')) r3=>x y. exact: logical_step_letinR.
 Qed.
 
-Lemma sta_conv_ifte A A' m m' n1 n1' n2 n2' :
+Lemma logical_conv_ifte A A' m m' n1 n1' n2 n2' :
   A ≃ A' -> m ≃ m' -> n1 ≃ n1' -> n2 ≃ n2' -> Ifte A m n1 n2 ≃ Ifte A' m' n1' n2'.
 Proof.
   move=>rA rm rn1 rn2.
   apply: (conv_trans (Ifte A' m n1 n2)).
-  apply: (conv_hom (((Ifte^~ m)^~ n1)^~ n2)) rA=>x y. exact: sta_step_ifteA.
+  apply: (conv_hom (((Ifte^~ m)^~ n1)^~ n2)) rA=>x y. exact: logical_step_ifteA.
   apply: (conv_trans (Ifte A' m' n1 n2)).
-  apply: (conv_hom (((Ifte A')^~ n1)^~ n2)) rm=>x y. exact: sta_step_ifteM.
+  apply: (conv_hom (((Ifte A')^~ n1)^~ n2)) rm=>x y. exact: logical_step_ifteM.
   apply: (conv_trans (Ifte A' m' n1' n2)).
-  apply: (conv_hom ((Ifte A' m')^~ n2)) rn1=>x y. exact: sta_step_ifteN1.
-  apply: (conv_hom (Ifte A' m' n1')) rn2=>x y. exact: sta_step_ifteN2.
+  apply: (conv_hom ((Ifte A' m')^~ n2)) rn1=>x y. exact: logical_step_ifteN1.
+  apply: (conv_hom (Ifte A' m' n1')) rn2=>x y. exact: logical_step_ifteN2.
 Qed.
 
-Lemma sta_conv_id A A' m m' n n' :
+Lemma logical_conv_id A A' m m' n n' :
   A ≃ A' -> m ≃ m' -> n ≃ n' -> Id A m n ≃ Id A' m' n'.
 Proof.
   move=>r1 r2 r3.
   apply: (conv_trans (Id A' m n)).
-  apply: (conv_hom ((Id^~ m)^~ n)) r1=>x y. exact: sta_step_idA.
+  apply: (conv_hom ((Id^~ m)^~ n)) r1=>x y. exact: logical_step_idA.
   apply: (conv_trans (Id A' m' n)).
-  apply: (conv_hom (Id A'^~ n)) r2=>x y. exact: sta_step_idL.
-  apply: (conv_hom (Id A' m')) r3=>x y. exact: sta_step_idR.
+  apply: (conv_hom (Id A'^~ n)) r2=>x y. exact: logical_step_idL.
+  apply: (conv_hom (Id A' m')) r3=>x y. exact: logical_step_idR.
 Qed.
 
-Lemma sta_conv_refl m m' :
+Lemma logical_conv_refl m m' :
   m ≃ m' -> Refl m ≃ Refl m'.
 Proof.
   move=>r.
-  apply: (conv_hom Refl) r=>x y. exact: sta_step_refl.
+  apply: (conv_hom Refl) r=>x y. exact: logical_step_refl.
 Qed.
 
-Lemma sta_conv_rw A A' H H' P P' :
+Lemma logical_conv_rw A A' H H' P P' :
   A ≃ A' -> H ≃ H' -> P ≃ P' -> Rw A H P ≃ Rw A' H' P'.
 Proof.
   move=>r1 r2 r3.
   apply: (conv_trans (Rw A' H P)).
-  apply: (conv_hom ((Rw^~ H)^~ P)) r1=>x y. exact: sta_step_rwA.
+  apply: (conv_hom ((Rw^~ H)^~ P)) r1=>x y. exact: logical_step_rwA.
   apply: (conv_trans (Rw A' H' P)).
-  apply: (conv_hom (Rw A'^~ P)) r2=>x y. exact: sta_step_rwH.
-  apply: (conv_hom (Rw A' H')) r3=>x y. exact: sta_step_rwP.
+  apply: (conv_hom (Rw A'^~ P)) r2=>x y. exact: logical_step_rwH.
+  apply: (conv_hom (Rw A' H')) r3=>x y. exact: logical_step_rwP.
 Qed.
 
-Lemma sta_conv_subst σ m n :
+Lemma logical_conv_subst σ m n :
   m ≃ n -> m.[σ] ≃ n.[σ].
 Proof.
   move=>c.
   apply: conv_hom c.
-  exact: sta_step_subst.
+  exact: logical_step_subst.
 Qed.
 
 Lemma sconv_up σ τ : sconv σ τ -> sconv (up σ) (up τ).
-Proof. move=> A [|x] //=. asimpl. exact: sta_conv_subst. Qed.
+Proof. move=> A [|x] //=. asimpl. exact: logical_conv_subst. Qed.
 
 Lemma sconv_upn n σ τ : sconv σ τ -> sconv (upn n σ) (upn n τ).
 Proof.
@@ -450,48 +450,48 @@ Proof.
 Qed.
 
 #[export] Hint Resolve
-  sta_conv_app
-  sta_conv_lam0 sta_conv_lam1
-  sta_conv_pi0 sta_conv_pi1
-  sta_conv_sig0 sta_conv_sig1
-  sta_conv_pair0 sta_conv_pair1
-  sta_conv_letin sta_conv_ifte
-  sta_conv_id sta_conv_refl sta_conv_rw
-  sconv_up sconv_upn : sta_conv_congr.
+  logical_conv_app
+  logical_conv_lam0 logical_conv_lam1
+  logical_conv_pi0 logical_conv_pi1
+  logical_conv_sig0 logical_conv_sig1
+  logical_conv_pair0 logical_conv_pair1
+  logical_conv_letin logical_conv_ifte
+  logical_conv_id logical_conv_refl logical_conv_rw
+  sconv_up sconv_upn : logical_conv_congr.
 
-Lemma sta_conv_compat σ τ s :
+Lemma logical_conv_compat σ τ s :
   sconv σ τ -> s.[σ] ≃ s.[τ].
-Proof. elim: s σ τ => *; asimpl; eauto 9 with sta_conv_congr. Qed.
+Proof. elim: s σ τ => *; asimpl; eauto 9 with logical_conv_congr. Qed.
 
-Lemma sta_conv_beta m n1 n2 : n1 ≃ n2 -> m.[n1/] ≃ m.[n2/].
-Proof. move=> c. by apply: sta_conv_compat => -[]. Qed.
+Lemma logical_conv_beta m n1 n2 : n1 ≃ n2 -> m.[n1/] ≃ m.[n2/].
+Proof. move=> c. by apply: logical_conv_compat => -[]. Qed.
 
 Lemma pstep_reflexive m : pstep m m.
 Proof. elim: m; eauto using pstep. Qed.
 #[global] Hint Resolve pstep_reflexive.
 
-Lemma sta_step_pstep m m' : sta_step m m' -> pstep m m'.
+Lemma logical_step_pstep m m' : logical_step m m' -> pstep m m'.
 Proof with eauto using pstep, pstep_reflexive. elim... Qed.
 
-Lemma pstep_sta_red m n : pstep m n -> m ~>* n.
+Lemma pstep_logical_red m n : pstep m n -> m ~>* n.
 Proof with eauto.
-  elim=>{m n}//=; eauto with sta_red_congr.
+  elim=>{m n}//=; eauto with logical_red_congr.
   { move=> A m m' n n' s p1 r1 p2 r2.
     apply: starES. by constructor.
-    apply: (star_trans (m'.[n/])). exact: sta_red_subst.
-    by apply: sta_red_compat=>-[|]. }
+    apply: (star_trans (m'.[n/])). exact: logical_red_subst.
+    by apply: logical_red_compat=>-[|]. }
   { move=> A m m' n n' s p1 r1 p2 r2.
     apply: starES. by constructor.
-    apply: (star_trans (m'.[n/])). exact: sta_red_subst.
-    by apply: sta_red_compat=>-[|]. }
+    apply: (star_trans (m'.[n/])). exact: logical_red_subst.
+    by apply: logical_red_compat=>-[|]. }
   { move=> A m1 m1' m2 m2' n n' s p1 r1 p2 r2 p r.
     apply: starES. by constructor.
-    apply: (star_trans (n'.[m2,m1/])). exact: sta_red_subst.
-    by apply: sta_red_compat=>-[|-[]]. }
+    apply: (star_trans (n'.[m2,m1/])). exact: logical_red_subst.
+    by apply: logical_red_compat=>-[|-[]]. }
   { move=> A m1 m1' m2 m2' n n' s p1 r1 p2 r2 p r.
     apply: starES. by constructor.
-    apply: (star_trans (n'.[m2,m1/])). exact: sta_red_subst.
-    by apply: sta_red_compat=>-[|-[]]. }
+    apply: (star_trans (n'.[m2,m1/])). exact: logical_red_subst.
+    by apply: logical_red_compat=>-[|-[]]. }
   { move=>m m' n s p r.
     apply: starES. by constructor. eauto. }
   { move=>m m' n s p r.
@@ -736,52 +736,52 @@ Lemma strip m m1 m2 :
   pstep m m1 -> m ~>* m2 -> exists2 m', m1 ~>* m' & pstep m2 m'.
 Proof with eauto using pstep_refl, star.
   move=>p r. elim: r m1 p=>{m2}...
-  move=>m1 m2 r1 ih /sta_step_pstep p1 m' p2.
+  move=>m1 m2 r1 ih /logical_step_pstep p1 m' p2.
   move:(ih _ p2)=>[m3 r2 p3].
   move:(pstep_diamond p1 p3)=>[m4 p4 p5].
   exists m4...
   apply: star_trans.
   apply: r2.
-  by apply: pstep_sta_red.
+  by apply: pstep_logical_red.
 Qed.
 
 Theorem confluence :
-  confluent sta_step.
-Proof with eauto using sta_step, star.
+  confluent logical_step.
+Proof with eauto using logical_step, star.
   unfold confluent.
   unfold joinable.
   move=> x y z r.
   elim: r z=>{y}.
   move=>z r. exists z...
-  move=>y z r1 ih /sta_step_pstep p z0 /ih[z1 r2 r3].
+  move=>y z r1 ih /logical_step_pstep p z0 /ih[z1 r2 r3].
   move:(strip p r2)=>[z2 r4 p1].
   exists z2...
   apply: star_trans.
   apply r3.
-  apply: pstep_sta_red...
+  apply: pstep_logical_red...
 Qed.
 
 Theorem church_rosser :
-  CR sta_step.
+  CR logical_step.
 Proof.
   apply confluent_cr.
   apply confluence.
 Qed.
 
-Lemma sta_red_var_inv x y : Var x ~>* y -> y = Var x.
+Lemma logical_red_var_inv x y : Var x ~>* y -> y = Var x.
 Proof.
   elim=>//{} y z r1 e r2; subst.
   inv r2.
 Qed.
 
-Lemma sta_red_sort_inv s l A :
+Lemma logical_red_sort_inv s l A :
   Sort s l ~>* A -> A = Sort s l.
 Proof.
   elim=>//y z r1 e r2; subst.
   inv r2.
 Qed.
 
-Lemma sta_red_pi0_inv A B s x :
+Lemma logical_red_pi0_inv A B s x :
   Pi0 A B s ~>* x ->
   exists A' B',
     A ~>* A' /\ B ~>* B' /\ x = Pi0 A' B' s.
@@ -798,7 +798,7 @@ Proof.
   apply: starSE; eauto.
 Qed.
 
-Lemma sta_red_pi1_inv A B s x :
+Lemma logical_red_pi1_inv A B s x :
   Pi1 A B s ~>* x ->
   exists A' B',
     A ~>* A' /\ B ~>* B' /\ x = Pi1 A' B' s.
@@ -815,7 +815,7 @@ Proof.
   apply: starSE; eauto.
 Qed.
 
-Lemma sta_red_lam0_inv A m x s :
+Lemma logical_red_lam0_inv A m x s :
   Lam0 A m s ~>* x ->
   exists A' m',
     A ~>* A' /\ m ~>* m' /\ x = Lam0 A' m' s.
@@ -828,7 +828,7 @@ Proof.
   exists A'. exists m'0. eauto using star.
 Qed.
 
-Lemma sta_red_lam1_inv A m x s :
+Lemma logical_red_lam1_inv A m x s :
   Lam1 A m s ~>* x ->
   exists A' m',
     A ~>* A' /\ m ~>* m' /\ x = Lam1 A' m' s.
@@ -841,7 +841,7 @@ Proof.
   exists A'. exists m'0. eauto using star.
 Qed.
 
-Lemma sta_red_sig0_inv A B s x :
+Lemma logical_red_sig0_inv A B s x :
   Sig0 A B s ~>* x ->
   exists A' B',
     A ~>* A' /\ B ~>* B' /\ x = Sig0 A' B' s.
@@ -858,7 +858,7 @@ Proof.
   apply: starSE; eauto.
 Qed.
 
-Lemma sta_red_sig1_inv A B s x :
+Lemma logical_red_sig1_inv A B s x :
   Sig1 A B s ~>* x ->
   exists A' B',
     A ~>* A' /\ B ~>* B' /\ x = Sig1 A' B' s.
@@ -875,7 +875,7 @@ Proof.
   apply: starSE; eauto.
 Qed.
 
-Lemma sta_red_pair0_inv m n s x :
+Lemma logical_red_pair0_inv m n s x :
   Pair0 m n s ~>* x ->
   exists m' n',
     m ~>* m' /\ n ~>* n' /\ x = Pair0 m' n' s.
@@ -892,7 +892,7 @@ Proof.
   apply: starSE; eauto.
 Qed.
 
-Lemma sta_red_pair1_inv m n s x :
+Lemma logical_red_pair1_inv m n s x :
   Pair1 m n s ~>* x ->
   exists m' n',
     m ~>* m' /\ n ~>* n' /\ x = Pair1 m' n' s.
@@ -909,28 +909,28 @@ Proof.
   apply: starSE; eauto.
 Qed.
 
-Lemma sta_red_bool_inv x : Bool ~>* x -> x = Bool.
+Lemma logical_red_bool_inv x : Bool ~>* x -> x = Bool.
 Proof.
   elim=>//.
   move=>y z rd e st. subst.
   inv st.
 Qed.
 
-Lemma sta_red_tt_inv x : TT ~>* x -> x = TT.
+Lemma logical_red_tt_inv x : TT ~>* x -> x = TT.
 Proof.
   elim=>//.
   move=>y z rd e st. subst.
   inv st.
 Qed.
 
-Lemma sta_red_ff_inv x : FF ~>* x -> x = FF.
+Lemma logical_red_ff_inv x : FF ~>* x -> x = FF.
 Proof.
   elim=>//.
   move=>y z rd e st. subst.
   inv st.
 Qed.
 
-Lemma sta_red_id_inv A m n x :
+Lemma logical_red_id_inv A m n x :
   Id A m n ~>* x ->
   exists A' m' n',
     A ~>* A' /\ m ~>* m' /\ n ~>* n' /\ x = Id A' m' n'.
@@ -950,7 +950,7 @@ Proof.
   apply: starSE; eauto.
 Qed.
 
-Lemma sta_red_refl_inv m x :
+Lemma logical_red_refl_inv m x :
   Refl m ~>* x ->
   exists m', m ~>* m' /\ x = Refl m'.
 Proof.
@@ -965,7 +965,7 @@ Qed.
 Lemma sort_inj s1 s2 l1 l2 :
   Sort s1 l1 ≃ Sort s2 l2 -> s1 = s2 /\ l1 = l2.
 Proof.
-  move/church_rosser=>[x/sta_red_sort_inv->/sta_red_sort_inv[->]]//.
+  move/church_rosser=>[x/logical_red_sort_inv->/logical_red_sort_inv[->]]//.
 Qed.
 
 Lemma pi0_inj A A' B B' s s' :
@@ -973,8 +973,8 @@ Lemma pi0_inj A A' B B' s s' :
     A ≃ A' /\ B ≃ B' /\ s = s'.
 Proof.
   move/church_rosser=>
-    [x/sta_red_pi0_inv[A1[B1[rA1[rB1->]]]]
-      /sta_red_pi0_inv[A2[B2[rA2[rB2[]]]]]] eA eB es; subst.
+    [x/logical_red_pi0_inv[A1[B1[rA1[rB1->]]]]
+      /logical_red_pi0_inv[A2[B2[rA2[rB2[]]]]]] eA eB es; subst.
   repeat split.
   apply: conv_trans.
   apply: star_conv. by apply: rA1.
@@ -989,8 +989,8 @@ Lemma pi1_inj A A' B B' s s' :
     A ≃ A' /\ B ≃ B' /\ s = s'.
 Proof.
   move/church_rosser=>
-    [x/sta_red_pi1_inv[A1[B1[rA1[rB1->]]]]
-      /sta_red_pi1_inv[A2[B2[rA2[rB2[]]]]]] eA eB es; subst.
+    [x/logical_red_pi1_inv[A1[B1[rA1[rB1->]]]]
+      /logical_red_pi1_inv[A2[B2[rA2[rB2[]]]]]] eA eB es; subst.
   repeat split.
   apply: conv_trans.
   apply: star_conv. by apply: rA1.
@@ -1005,8 +1005,8 @@ Lemma sig0_inj A A' B B' s s' :
     A ≃ A' /\ B ≃ B' /\ s = s'.
 Proof.
   move/church_rosser=>
-    [x/sta_red_sig0_inv[A1[B1[rA1[rB1->]]]]
-      /sta_red_sig0_inv[A2[B2[rA2[rB2[]]]]]] eA eB es; subst.
+    [x/logical_red_sig0_inv[A1[B1[rA1[rB1->]]]]
+      /logical_red_sig0_inv[A2[B2[rA2[rB2[]]]]]] eA eB es; subst.
   repeat split.
   apply: conv_trans.
   apply: star_conv. by apply: rA1.
@@ -1021,8 +1021,8 @@ Lemma sig1_inj A A' B B' s s' :
     A ≃ A' /\ B ≃ B' /\ s = s'.
 Proof.
   move/church_rosser=>
-    [x/sta_red_sig1_inv[A1[B1[rA1[rB1->]]]]
-      /sta_red_sig1_inv[A2[B2[rA2[rB2[]]]]]] eA eB es; subst.
+    [x/logical_red_sig1_inv[A1[B1[rA1[rB1->]]]]
+      /logical_red_sig1_inv[A2[B2[rA2[rB2[]]]]]] eA eB es; subst.
   repeat split.
   apply: conv_trans.
   apply: star_conv. by apply: rA1.
@@ -1037,8 +1037,8 @@ Lemma id_inj A A' m m' n n' :
     A ≃ A' /\ m ≃ m' /\ n ≃ n'.
 Proof.
   move/church_rosser=>
-    [x/sta_red_id_inv[A1[m1[n1[rA1[rm1[rn1->]]]]]]
-      /sta_red_id_inv[A2[m2[n2[rA2[rm2[rn2[]]]]]]]] eA em en; subst.
+    [x/logical_red_id_inv[A1[m1[n1[rA1[rm1[rn1->]]]]]]
+      /logical_red_id_inv[A2[m2[n2[rA2[rm2[rn2[]]]]]]]] eA em en; subst.
   repeat split.
   apply: conv_trans.
   apply: star_conv. by apply: rA1.
@@ -1053,21 +1053,21 @@ Qed.
 
 Ltac red_inv m H :=
   match m with
-  | Var   => apply sta_red_var_inv in H
-  | Sort  => apply sta_red_sort_inv in H
-  | Pi0   => apply sta_red_pi0_inv in H
-  | Pi1   => apply sta_red_pi1_inv in H
-  | Lam0  => apply sta_red_lam0_inv in H
-  | Lam1  => apply sta_red_lam1_inv in H
-  | Sig0  => apply sta_red_sig0_inv in H
-  | Sig1  => apply sta_red_sig1_inv in H
-  | Pair0 => apply sta_red_pair0_inv in H
-  | Pair1 => apply sta_red_pair1_inv in H
-  | Bool  => apply sta_red_bool_inv in H
-  | TT    => apply sta_red_tt_inv in H
-  | FF    => apply sta_red_ff_inv in H
-  | Id    => apply sta_red_id_inv in H
-  | Refl  => apply sta_red_refl_inv in H
+  | Var   => apply logical_red_var_inv in H
+  | Sort  => apply logical_red_sort_inv in H
+  | Pi0   => apply logical_red_pi0_inv in H
+  | Pi1   => apply logical_red_pi1_inv in H
+  | Lam0  => apply logical_red_lam0_inv in H
+  | Lam1  => apply logical_red_lam1_inv in H
+  | Sig0  => apply logical_red_sig0_inv in H
+  | Sig1  => apply logical_red_sig1_inv in H
+  | Pair0 => apply logical_red_pair0_inv in H
+  | Pair1 => apply logical_red_pair1_inv in H
+  | Bool  => apply logical_red_bool_inv in H
+  | TT    => apply logical_red_tt_inv in H
+  | FF    => apply logical_red_ff_inv in H
+  | Id    => apply logical_red_id_inv in H
+  | Refl  => apply logical_red_refl_inv in H
   end.
 
 Ltac solve_conv' :=
@@ -1077,12 +1077,12 @@ Ltac solve_conv' :=
     apply church_rosser in H; inv H
   end;
   repeat match goal with
-  | [ H : sta_red (?m _) _ |- _ ]         => red_inv m H
-  | [ H : sta_red (?m _ _) _ |- _ ]       => red_inv m H
-  | [ H : sta_red (?m _ _ _) _ |- _ ]     => red_inv m H
-  | [ H : sta_red (?m _ _ _ _) _ |- _ ]   => red_inv m H
-  | [ H : sta_red (?m _ _ _ _ _) _ |- _ ] => red_inv m H
-  | [ H : sta_red ?m _ |- _ ]             => red_inv m H
+  | [ H : logical_red (?m _) _ |- _ ]         => red_inv m H
+  | [ H : logical_red (?m _ _) _ |- _ ]       => red_inv m H
+  | [ H : logical_red (?m _ _ _) _ |- _ ]     => red_inv m H
+  | [ H : logical_red (?m _ _ _ _) _ |- _ ]   => red_inv m H
+  | [ H : logical_red (?m _ _ _ _ _) _ |- _ ] => red_inv m H
+  | [ H : logical_red ?m _ |- _ ]             => red_inv m H
   end;
   firstorder; subst;
   match goal with
