coq/theories/logical_type.v
@@ -1,250 +1,250 @@
 From mathcomp Require Import ssreflect ssrbool eqtype ssrnat seq.
 From Stdlib Require Import ssrfun Classical Utf8.
-Require Export AutosubstSsr ARS sta_ctx sta_step.
+Require Export AutosubstSsr ARS logical_ctx logical_step.
 
 Set Implicit Arguments.
 Unset Strict Implicit.
 Unset Printing Implicit Defensive.
 
-Inductive sta0_type : sta_ctx -> term -> term -> Prop :=
-| sta0_axiom Γ s l :
-  sta0_wf Γ ->
-  sta0_type Γ (Sort s l) (Sort U l.+1)
-| sta0_var Γ x A :
-  sta0_wf Γ ->
-  sta_has Γ x A ->
-  sta0_type Γ (Var x) A
-| sta0_pi0 Γ A B s r t l1 l2 :
-  sta0_type Γ A (Sort r l1) ->
-  sta0_type (A :: Γ) B (Sort t l2) ->
-  sta0_type Γ (Pi0 A B s) (Sort s (maxn l1 l2))
-| sta0_pi1 Γ A B s r t l1 l2 :
-  sta0_type Γ A (Sort r l1) ->
-  sta0_type (A :: Γ) B (Sort t l2) ->
-  sta0_type Γ (Pi1 A B s) (Sort s (maxn l1 l2))
-| sta0_lam0 Γ A B m s r l :
-  sta0_type Γ A (Sort r l) ->
-  sta0_type (A :: Γ) m B ->
-  sta0_type Γ (Lam0 A m s) (Pi0 A B s)
-| sta0_lam1 Γ A B m s r l :
-  sta0_type Γ A (Sort r l) ->
-  sta0_type (A :: Γ) m B ->
-  sta0_type Γ (Lam1 A m s) (Pi1 A B s)
-| sta0_app0 Γ A B m n s :
-  sta0_type Γ m (Pi0 A B s) ->
-  sta0_type Γ n A ->
-  sta0_type Γ (App m n) B.[n/]
-| sta0_app1 Γ A B m n s :
-  sta0_type Γ m (Pi1 A B s) ->
-  sta0_type Γ n A ->
-  sta0_type Γ (App m n) B.[n/]
-| sta0_sig0 Γ A B s r t l1 l2 :
+Inductive logical0_type : logical_ctx -> term -> term -> Prop :=
+| logical0_axiom Γ s l :
+  logical0_wf Γ ->
+  logical0_type Γ (Sort s l) (Sort U l.+1)
+| logical0_var Γ x A :
+  logical0_wf Γ ->
+  logical_has Γ x A ->
+  logical0_type Γ (Var x) A
+| logical0_pi0 Γ A B s r t l1 l2 :
+  logical0_type Γ A (Sort r l1) ->
+  logical0_type (A :: Γ) B (Sort t l2) ->
+  logical0_type Γ (Pi0 A B s) (Sort s (maxn l1 l2))
+| logical0_pi1 Γ A B s r t l1 l2 :
+  logical0_type Γ A (Sort r l1) ->
+  logical0_type (A :: Γ) B (Sort t l2) ->
+  logical0_type Γ (Pi1 A B s) (Sort s (maxn l1 l2))
+| logical0_lam0 Γ A B m s r l :
+  logical0_type Γ A (Sort r l) ->
+  logical0_type (A :: Γ) m B ->
+  logical0_type Γ (Lam0 A m s) (Pi0 A B s)
+| logical0_lam1 Γ A B m s r l :
+  logical0_type Γ A (Sort r l) ->
+  logical0_type (A :: Γ) m B ->
+  logical0_type Γ (Lam1 A m s) (Pi1 A B s)
+| logical0_app0 Γ A B m n s :
+  logical0_type Γ m (Pi0 A B s) ->
+  logical0_type Γ n A ->
+  logical0_type Γ (App m n) B.[n/]
+| logical0_app1 Γ A B m n s :
+  logical0_type Γ m (Pi1 A B s) ->
+  logical0_type Γ n A ->
+  logical0_type Γ (App m n) B.[n/]
+| logical0_sig0 Γ A B s r t l1 l2 :
   s ⊑ t ->
-  sta0_type Γ A (Sort s l1) ->
-  sta0_type (A :: Γ) B (Sort r l2) ->
-  sta0_type Γ (Sig0 A B t) (Sort t (maxn l1 l2))
-| sta0_sig1 Γ A B s r t l1 l2 :
+  logical0_type Γ A (Sort s l1) ->
+  logical0_type (A :: Γ) B (Sort r l2) ->
+  logical0_type Γ (Sig0 A B t) (Sort t (maxn l1 l2))
+| logical0_sig1 Γ A B s r t l1 l2 :
   s ⊑ t ->
   r ⊑ t ->
-  sta0_type Γ A (Sort s l1) ->
-  sta0_type (A :: Γ) B (Sort r l2) ->
-  sta0_type Γ (Sig1 A B t) (Sort t (maxn l1 l2))
-| sta0_pair0 Γ A B m n t l :
-  sta0_type Γ (Sig0 A B t) (Sort t l) ->
-  sta0_type Γ m A ->
-  sta0_type Γ n B.[m/] ->
-  sta0_type Γ (Pair0 m n t) (Sig0 A B t)
-| sta0_pair1 Γ A B m n t l :
-  sta0_type Γ (Sig1 A B t) (Sort t l) ->
-  sta0_type Γ m A ->
-  sta0_type Γ n B.[m/] ->
-  sta0_type Γ (Pair1 m n t) (Sig1 A B t)
-| sta0_letin0 Γ A B C m n s t l :
-  sta0_type (Sig0 A B t :: Γ) C (Sort s l) ->
-  sta0_type Γ m (Sig0 A B t) ->
-  sta0_type (B :: A :: Γ) n C.[Pair0 (Var 1) (Var 0) t .: ren (+2)] ->
-  sta0_type Γ (LetIn C m n) C.[m/]
-| sta0_letin1 Γ A B C m n s t l :
-  sta0_type (Sig1 A B t :: Γ) C (Sort s l) ->
-  sta0_type Γ m (Sig1 A B t) ->
-  sta0_type (B :: A :: Γ) n C.[Pair1 (Var 1) (Var 0) t .: ren (+2)] ->
-  sta0_type Γ (LetIn C m n) C.[m/]
-| sta0_bool Γ :
-  sta0_wf Γ ->
-  sta0_type Γ Bool (Sort U 0)
-| sta0_tt Γ :
-  sta0_wf Γ ->
-  sta0_type Γ TT Bool
-| sta0_ff Γ :
-  sta0_wf Γ ->
-  sta0_type Γ FF Bool
-| sta0_ifte Γ A m n1 n2 s l :
-  sta0_type (Bool :: Γ) A (Sort s l) ->
-  sta0_type Γ m Bool ->
-  sta0_type Γ n1 A.[TT/] ->
-  sta0_type Γ n2 A.[FF/] ->
-  sta0_type Γ (Ifte A m n1 n2) A.[m/]
-| sta0_id Γ A m n s l :
-  sta0_type Γ A (Sort s l) ->
-  sta0_type Γ m A ->
-  sta0_type Γ n A ->
-  sta0_type Γ (Id A m n) (Sort U l)
-| sta0_refl Γ A m :
-  sta0_type Γ m A ->
-  sta0_type Γ (Refl m) (Id A m m)
-| sta0_rw Γ A B H P m n s l :
-  sta0_type (Id A.[ren (+1)] m.[ren (+1)] (Var 0) :: A :: Γ) B (Sort s l) ->
-  sta0_type Γ H B.[Refl m,m/] ->
-  sta0_type Γ P (Id A m n) ->
-  sta0_type Γ (Rw B H P) B.[P,n/]
-| sta0_conv Γ A B m s l :
+  logical0_type Γ A (Sort s l1) ->
+  logical0_type (A :: Γ) B (Sort r l2) ->
+  logical0_type Γ (Sig1 A B t) (Sort t (maxn l1 l2))
+| logical0_pair0 Γ A B m n t l :
+  logical0_type Γ (Sig0 A B t) (Sort t l) ->
+  logical0_type Γ m A ->
+  logical0_type Γ n B.[m/] ->
+  logical0_type Γ (Pair0 m n t) (Sig0 A B t)
+| logical0_pair1 Γ A B m n t l :
+  logical0_type Γ (Sig1 A B t) (Sort t l) ->
+  logical0_type Γ m A ->
+  logical0_type Γ n B.[m/] ->
+  logical0_type Γ (Pair1 m n t) (Sig1 A B t)
+| logical0_letin0 Γ A B C m n s t l :
+  logical0_type (Sig0 A B t :: Γ) C (Sort s l) ->
+  logical0_type Γ m (Sig0 A B t) ->
+  logical0_type (B :: A :: Γ) n C.[Pair0 (Var 1) (Var 0) t .: ren (+2)] ->
+  logical0_type Γ (LetIn C m n) C.[m/]
+| logical0_letin1 Γ A B C m n s t l :
+  logical0_type (Sig1 A B t :: Γ) C (Sort s l) ->
+  logical0_type Γ m (Sig1 A B t) ->
+  logical0_type (B :: A :: Γ) n C.[Pair1 (Var 1) (Var 0) t .: ren (+2)] ->
+  logical0_type Γ (LetIn C m n) C.[m/]
+| logical0_bool Γ :
+  logical0_wf Γ ->
+  logical0_type Γ Bool (Sort U 0)
+| logical0_tt Γ :
+  logical0_wf Γ ->
+  logical0_type Γ TT Bool
+| logical0_ff Γ :
+  logical0_wf Γ ->
+  logical0_type Γ FF Bool
+| logical0_ifte Γ A m n1 n2 s l :
+  logical0_type (Bool :: Γ) A (Sort s l) ->
+  logical0_type Γ m Bool ->
+  logical0_type Γ n1 A.[TT/] ->
+  logical0_type Γ n2 A.[FF/] ->
+  logical0_type Γ (Ifte A m n1 n2) A.[m/]
+| logical0_id Γ A m n s l :
+  logical0_type Γ A (Sort s l) ->
+  logical0_type Γ m A ->
+  logical0_type Γ n A ->
+  logical0_type Γ (Id A m n) (Sort U l)
+| logical0_refl Γ A m :
+  logical0_type Γ m A ->
+  logical0_type Γ (Refl m) (Id A m m)
+| logical0_rw Γ A B H P m n s l :
+  logical0_type (Id A.[ren (+1)] m.[ren (+1)] (Var 0) :: A :: Γ) B (Sort s l) ->
+  logical0_type Γ H B.[Refl m,m/] ->
+  logical0_type Γ P (Id A m n) ->
+  logical0_type Γ (Rw B H P) B.[P,n/]
+| logical0_conv Γ A B m s l :
   A ≃ B ->
-  sta0_type Γ m A ->
-  sta0_type Γ B (Sort s l) ->
-  sta0_type Γ m B
+  logical0_type Γ m A ->
+  logical0_type Γ B (Sort s l) ->
+  logical0_type Γ m B
 
-with sta0_wf : sta_ctx -> Prop :=
-| sta0_wf_nil : sta0_wf nil
-| sta0_wf_cons Γ A s l :
-  sta0_wf Γ ->
-  sta0_type Γ A (Sort s l) ->
-  sta0_wf (A :: Γ).
+with logical0_wf : logical_ctx -> Prop :=
+| logical0_wf_nil : logical0_wf nil
+| logical0_wf_cons Γ A s l :
+  logical0_wf Γ ->
+  logical0_type Γ A (Sort s l) ->
+  logical0_wf (A :: Γ).
 
-Scheme sta0_type_mut := Induction for sta0_type Sort Prop
-with sta0_wf_mut := Induction for sta0_wf Sort Prop.
+Scheme logical0_type_mut := Induction for logical0_type Sort Prop
+with logical0_wf_mut := Induction for logical0_wf Sort Prop.
 
-Lemma sta0_type_wf Γ m A : sta0_type Γ m A -> sta0_wf Γ.
+Lemma logical0_type_wf Γ m A : logical0_type Γ m A -> logical0_wf Γ.
 Proof with eauto. elim=>{Γ m A}... Qed.
-#[global] Hint Resolve sta0_type_wf.
+#[global] Hint Resolve logical0_type_wf.
 
 Reserved Notation "Γ ⊢ m : A" (at level 50, m, A at next level).
-Inductive sta_type : sta_ctx -> term -> term -> Prop :=
-| sta_axiom Γ s l :
-  sta_wf Γ ->
+Inductive logical_type : logical_ctx -> term -> term -> Prop :=
+| logical_axiom Γ s l :
+  logical_wf Γ ->
   Γ ⊢ Sort s l : Sort U l.+1
-| sta_var Γ x A :
-  sta_wf Γ ->
-  sta_has Γ x A ->
+| logical_var Γ x A :
+  logical_wf Γ ->
+  logical_has Γ x A ->
   Γ ⊢ Var x : A
-| sta_pi0 Γ A B s r t l1 l2 :
+| logical_pi0 Γ A B s r t l1 l2 :
   Γ ⊢ A : Sort r l1 ->
   (A :: Γ) ⊢ B : Sort t l2 ->
   Γ ⊢ Pi0 A B s : Sort s (maxn l1 l2)
-| sta_pi1 Γ A B s r t l1 l2 :
+| logical_pi1 Γ A B s r t l1 l2 :
   Γ ⊢ A : Sort r l1 ->
   (A :: Γ) ⊢ B : Sort t l2 ->
   Γ ⊢ Pi1 A B s : Sort s (maxn l1 l2)
-| sta_lam0 Γ A B m s :
+| logical_lam0 Γ A B m s :
   (A :: Γ) ⊢ m : B ->
   Γ ⊢ Lam0 A m s : Pi0 A B s
-| sta_lam1 Γ A B m s :
+| logical_lam1 Γ A B m s :
   (A :: Γ) ⊢ m : B ->
   Γ ⊢ Lam1 A m s : Pi1 A B s
-| sta_app0 Γ A B m n s :
+| logical_app0 Γ A B m n s :
   Γ ⊢ m : Pi0 A B s ->
   Γ ⊢ n : A ->
   Γ ⊢ App m n : B.[n/]
-| sta_app1 Γ A B m n s :
+| logical_app1 Γ A B m n s :
   Γ ⊢ m : Pi1 A B s ->
   Γ ⊢ n : A ->
   Γ ⊢ App m n : B.[n/]
-| sta_sig0 Γ A B s r t l1 l2 :
+| logical_sig0 Γ A B s r t l1 l2 :
   s ⊑ t ->
   Γ ⊢ A : Sort s l1 ->
   (A :: Γ) ⊢ B : Sort r l2 ->
   Γ ⊢ Sig0 A B t : Sort t (maxn l1 l2)
-| sta_sig1 Γ A B s r t l1 l2 :
+| logical_sig1 Γ A B s r t l1 l2 :
   s ⊑ t ->
   r ⊑ t ->
   Γ ⊢ A : Sort s l1 ->
   (A :: Γ) ⊢ B : Sort r l2 ->
   Γ ⊢ Sig1 A B t : Sort t (maxn l1 l2)
-| sta_pair0 Γ A B m n t l :
+| logical_pair0 Γ A B m n t l :
   Γ ⊢ Sig0 A B t : Sort t l ->
   Γ ⊢ m : A ->
   Γ ⊢ n : B.[m/] ->
   Γ ⊢ Pair0 m n t : Sig0 A B t
-| sta_pair1 Γ A B m n t l :
+| logical_pair1 Γ A B m n t l :
   Γ ⊢ Sig1 A B t : Sort t l ->
   Γ ⊢ m : A ->
   Γ ⊢ n : B.[m/] ->
   Γ ⊢ Pair1 m n t : Sig1 A B t
-| sta_letin0 Γ A B C m n s t l :
+| logical_letin0 Γ A B C m n s t l :
   (Sig0 A B t :: Γ) ⊢ C : Sort s l ->
   Γ ⊢ m : Sig0 A B t ->
   (B :: A :: Γ) ⊢ n : C.[Pair0 (Var 1) (Var 0) t .: ren (+2)] ->
   Γ ⊢ LetIn C m n : C.[m/]
-| sta_letin1 Γ A B C m n s t l :
+| logical_letin1 Γ A B C m n s t l :
   (Sig1 A B t :: Γ) ⊢ C : Sort s l ->
   Γ ⊢ m : Sig1 A B t ->
   (B :: A :: Γ) ⊢ n : C.[Pair1 (Var 1) (Var 0) t .: ren (+2)] ->
   Γ ⊢ LetIn C m n : C.[m/]
-| sta_bool Γ :
-  sta_wf Γ ->
+| logical_bool Γ :
+  logical_wf Γ ->
   Γ ⊢ Bool : Sort U 0
-| sta_tt Γ :
-  sta_wf Γ ->
+| logical_tt Γ :
+  logical_wf Γ ->
   Γ ⊢ TT : Bool
-| sta_ff Γ :
-  sta_wf Γ ->
+| logical_ff Γ :
+  logical_wf Γ ->
   Γ ⊢ FF : Bool
-| sta_ifte Γ A m n1 n2 s l :
+| logical_ifte Γ A m n1 n2 s l :
   (Bool :: Γ) ⊢ A : Sort s l ->
   Γ ⊢ m : Bool ->
   Γ ⊢ n1 : A.[TT/] ->
   Γ ⊢ n2 : A.[FF/] ->
   Γ ⊢ Ifte A m n1 n2 : A.[m/]
-| sta_id Γ A m n s l :
+| logical_id Γ A m n s l :
   Γ ⊢ A : Sort s l ->
   Γ ⊢ m : A ->
   Γ ⊢ n : A ->
   Γ ⊢ Id A m n : Sort U l
-| sta_refl Γ A m :
+| logical_refl Γ A m :
   Γ ⊢ m : A ->
   Γ ⊢ Refl m : Id A m m
-| sta_rw Γ A B H P m n s l :
+| logical_rw Γ A B H P m n s l :
   (Id A.[ren (+1)] m.[ren (+1)] (Var 0) :: A :: Γ) ⊢ B : Sort s l ->
   Γ ⊢ H : B.[Refl m,m/] ->
   Γ ⊢ P : Id A m n ->
   Γ ⊢ Rw B H P : B.[P,n/]
-| sta_conv Γ A B m s l :
+| logical_conv Γ A B m s l :
   A ≃ B ->
   Γ ⊢ m : A ->
   Γ ⊢ B : Sort s l ->
   Γ ⊢ m : B
-where "Γ ⊢ m : A" := (sta_type Γ m A)
+where "Γ ⊢ m : A" := (logical_type Γ m A)
 
-with sta_wf : sta_ctx -> Prop :=
-| sta_wf_nil : sta_wf nil
-| sta_wf_cons Γ A s l :
-  sta_wf Γ ->
+with logical_wf : logical_ctx -> Prop :=
+| logical_wf_nil : logical_wf nil
+| logical_wf_cons Γ A s l :
+  logical_wf Γ ->
   Γ ⊢ A : Sort s l ->
-  sta_wf (A :: Γ).
+  logical_wf (A :: Γ).
 
-Scheme sta_type_mut := Induction for sta_type Sort Prop
-with sta_wf_mut := Induction for sta_wf Sort Prop.
+Scheme logical_type_mut := Induction for logical_type Sort Prop
+with logical_wf_mut := Induction for logical_wf Sort Prop.
 
-Lemma sta_type_wf Γ m A : Γ ⊢ m : A -> sta_wf Γ.
+Lemma logical_type_wf Γ m A : Γ ⊢ m : A -> logical_wf Γ.
 Proof with eauto.
   elim=>{Γ m A}...
   { move=>Γ A _ _ _ _ wf. inv wf... }
   { move=>Γ A _ _ _ _ wf. inv wf... }
 Qed.
-#[global] Hint Resolve sta_type_wf.
+#[global] Hint Resolve logical_type_wf.
 
-Lemma sta_sta0_type Γ m A : Γ ⊢ m : A -> sta0_type Γ m A.
-Proof with eauto using sta0_type, sta0_wf.
-  move:Γ m A. apply:(@sta_type_mut _ (fun Γ wf => sta0_wf Γ))...
+Lemma logical_logical0_type Γ m A : Γ ⊢ m : A -> logical0_type Γ m A.
+Proof with eauto using logical0_type, logical0_wf.
+  move:Γ m A. apply:(@logical_type_mut _ (fun Γ wf => logical0_wf Γ))...
   { move=>Γ A B m s tym ihm.
-    have wf0:=sta0_type_wf ihm. inv wf0.
-    apply: sta0_lam0... }
+    have wf0:=logical0_type_wf ihm. inv wf0.
+    apply: logical0_lam0... }
   { move=>Γ A B m s tym ihm.
-    have wf0:=sta0_type_wf ihm. inv wf0.
-    apply: sta0_lam1... }
+    have wf0:=logical0_type_wf ihm. inv wf0.
+    apply: logical0_lam1... }
 Qed.
-#[global] Hint Resolve sta_sta0_type.
+#[global] Hint Resolve logical_logical0_type.
 
-Lemma sta0_sta_type Γ m A : sta0_type Γ m A -> Γ ⊢ m : A.
-Proof with eauto using sta_type, sta_wf.
-  move:Γ m A. apply:(@sta0_type_mut _ (fun Γ wf => sta_wf Γ))...
+Lemma logical0_logical_type Γ m A : logical0_type Γ m A -> Γ ⊢ m : A.
+Proof with eauto using logical_type, logical_wf.
+  move:Γ m A. apply:(@logical0_type_mut _ (fun Γ wf => logical_wf Γ))...
 Qed.
