coq/theories/erasure_inv.v
@@ -1,12 +1,12 @@
 From mathcomp Require Import ssreflect ssrbool eqtype ssrnat seq.
 From Stdlib Require Import ssrfun Classical Utf8.
-Require Export AutosubstSsr ARS era_subst.
+Require Export AutosubstSsr ARS erasure_subst.
 
 Set Implicit Arguments.
 Unset Strict Implicit.
 Unset Printing Implicit Defensive.
 
-Lemma era_var_form Γ Δ m x B :
+Lemma erasure_var_form Γ Δ m x B :
   Γ ; Δ ⊢ m ~ Var x : B -> exists x, m = Var x.
 Proof.
   move e:(Var x)=>n er. elim: er x e=>//{Γ Δ m n B}.
@@ -14,7 +14,7 @@ Proof.
   by exists x.
 Qed.
 
-Lemma era_lam0_form Γ Δ m n X B s :
+Lemma erasure_lam0_form Γ Δ m n X B s :
   Γ ; Δ ⊢ m ~ Lam0 X n s : B -> exists A n, m = Lam0 A n s.
 Proof.
   move e:(Lam0 X n s)=>x er. elim: er X n s e=>//{Γ Δ m x B}.
@@ -22,7 +22,7 @@ Proof.
   exists A. by exists m.
 Qed.
 
-Lemma era_lam1_form Γ Δ m n X B s :
+Lemma erasure_lam1_form Γ Δ m n X B s :
   Γ ; Δ ⊢ m ~ Lam1 X n s : B -> exists A n, m = Lam1 A n s.
 Proof.
   move e:(Lam1 X n s)=>x er. elim: er X n s e=>//{Γ Δ m x B}.
@@ -30,7 +30,7 @@ Proof.
   exists A. by exists m.
 Qed.
 
-Lemma era_pair0_form Γ Δ m m1' m2' A s :
+Lemma erasure_pair0_form Γ Δ m m1' m2' A s :
   Γ ; Δ ⊢ m ~ Pair0 m1' m2' s : A -> exists m1 m2, m = Pair0 m1 m2 s.
 Proof.
   move e:(Pair0 m1' m2' s)=>x er. elim: er m1' m2' s e=>//{Γ Δ m x A}.
@@ -38,7 +38,7 @@ Proof.
   exists m. by exists n.
 Qed.
 
-Lemma era_pair1_form Γ Δ m m1' m2' A s :
+Lemma erasure_pair1_form Γ Δ m m1' m2' A s :
   Γ ; Δ ⊢ m ~ Pair1 m1' m2' s : A -> exists m1 m2, m = Pair1 m1 m2 s.
 Proof.
   move e:(Pair1 m1' m2' s)=>x er. elim: er m1' m2' s e=>//{Γ Δ m x A}.
@@ -46,16 +46,16 @@ Proof.
   exists m. by exists n.
 Qed.
 
-Lemma era_tt_form Γ Δ m A : Γ ; Δ ⊢ m ~ TT : A -> m = TT.
+Lemma erasure_tt_form Γ Δ m A : Γ ; Δ ⊢ m ~ TT : A -> m = TT.
 Proof. move e:(TT)=>x er. elim: er e=>//. Qed.
 
-Lemma era_ff_form Γ Δ m A : Γ ; Δ ⊢ m ~ FF : A -> m = FF.
+Lemma erasure_ff_form Γ Δ m A : Γ ; Δ ⊢ m ~ FF : A -> m = FF.
 Proof. move e:(FF)=>x er. elim: er e=>//. Qed.
 
-Lemma era_box_form Γ Δ m A : ~Γ ; Δ ⊢ m ~ Box : A.
+Lemma erasure_box_form Γ Δ m A : ~Γ ; Δ ⊢ m ~ Box : A.
 Proof. move e:(Box)=>m' ty. elim: ty e=>//{Γ Δ m m' A}. Qed.
 
-Lemma era_lam0_invX Γ Δ A1 A2 A3 B C m1 m2 s1 s2 t l :
+Lemma erasure_lam0_invX Γ Δ A1 A2 A3 B C m1 m2 s1 s2 t l :
   Γ ; Δ ⊢ Lam0 A1 m1 s1 ~ Lam0 A2 m2 s1 : C ->
   C ≃ Pi0 A3 B s2 ->
   (A3 :: Γ) ⊢ B : Sort t l ->
@@ -67,9 +67,9 @@ Proof with eauto.
   { move=>Γ Δ A B m m' s k tym ihm A1 A2 A3 B0 m1 m2
       s1 s2 t l[e1 e2 e3][e5 e6 _]; subst.
     move=>/pi0_inj[eq1[eq2 e]]tyB0; subst.
-    have wf:=sta_type_wf tyB0. inv wf. split...
-    apply: era_conv...
-    apply: era_ctx_conv0.
+    have wf:=logical_type_wf tyB0. inv wf. split...
+    apply: erasure_conv...
+    apply: erasure_ctx_conv0.
     exact: (conv_sym eq1).
     exact: H2.
     exact: tym. }
@@ -79,7 +79,7 @@ Proof with eauto.
     apply: conv_trans... }
 Qed.
 
-Lemma era_lam1_invX Γ Δ A1 A2 A3 B C m1 m2 s1 s2 t l :
+Lemma erasure_lam1_invX Γ Δ A1 A2 A3 B C m1 m2 s1 s2 t l :
   Γ ; Δ ⊢ Lam1 A1 m1 s1 ~ Lam1 A2 m2 s1 : C ->
   C ≃ Pi1 A3 B s2 ->
   (A3 :: Γ) ⊢ B : Sort t l ->
@@ -91,43 +91,43 @@ Proof with eauto.
   { move=>Γ Δ A B m m' s t k tym ihm A1 A2 A3 B0 m1 m2
       s1 s2 t0 l0[e1 e2 e3][e5 e6 _]; subst.
     move=>/pi1_inj[eq1[eq2 e]]tyB0; subst.
-    have wf:=dyn_type_wf (era_dyn_type tym). inv wf.
-    have wf:=sta_type_wf tyB0. inv wf.
+    have wf:=program_type_wf (erasure_program_type tym). inv wf.
+    have wf:=logical_type_wf tyB0. inv wf.
     have[A0 rd1 rd2]:=church_rosser eq1.
-    have tyA0t:=sta_rd H4 rd1.
-    have tyA0s:=sta_rd H3 rd2.
-    have e:=sta_unicity tyA0t tyA0s. subst.
+    have tyA0t:=logical_rd H4 rd1.
+    have tyA0s:=logical_rd H3 rd2.
+    have e:=logical_unicity tyA0t tyA0s. subst.
     exists s. split...
-    apply: era_ctx_conv1.
+    apply: erasure_ctx_conv1.
     apply: conv_sym...
     exact: H3.
-    apply: era_conv...
-    apply: sta_ctx_conv... }
+    apply: erasure_conv...
+    apply: logical_ctx_conv... }
   { move=>Γ Δ A B m m' s l eq1 tym ihm tyB A1 A2 A3 B0 m1 m2
       s1 s2 t l0 e1 e2 eq tyB0; subst.
     apply: ihm...
     apply: conv_trans... }
 Qed.
 
-Lemma era_lam0_inv Γ Δ m m' A1 A2 A3 B s1 s2 :
+Lemma erasure_lam0_inv Γ Δ m m' A1 A2 A3 B s1 s2 :
   Γ ; Δ ⊢ Lam0 A1 m s2 ~ Lam0 A2 m' s2 : Pi0 A3 B s1 ->
   (A3 :: Γ) ; _: Δ ⊢ m ~ m' : B /\ A1 ≃ A3.
 Proof with eauto.
   move=>ty.
-  have[t[l/sta_pi0_inv[r[l1[l2[tyB _]]]]]]:=dyn_valid (era_dyn_type ty).
-  apply: era_lam0_invX...
+  have[t[l/logical_pi0_inv[r[l1[l2[tyB _]]]]]]:=program_valid (erasure_program_type ty).
+  apply: erasure_lam0_invX...
 Qed.
 
-Lemma era_lam1_inv Γ Δ m m' A1 A2 A3 B s1 s2 :
+Lemma erasure_lam1_inv Γ Δ m m' A1 A2 A3 B s1 s2 :
   Γ ; Δ ⊢ Lam1 A1 m s2 ~ Lam1 A2 m' s2 : Pi1 A3 B s1 ->
   exists r, (A3 :: Γ) ; A3 .{r} Δ ⊢ m ~ m' : B /\ A1 ≃ A3.
 Proof with eauto.
   move=>ty.
-  have[t[l/sta_pi1_inv[r[l1[l2[tyB _]]]]]]:=dyn_valid (era_dyn_type ty).
-  apply: era_lam1_invX...
+  have[t[l/logical_pi1_inv[r[l1[l2[tyB _]]]]]]:=program_valid (erasure_program_type ty).
+  apply: erasure_lam1_invX...
 Qed.
 
-Lemma era_pair0_invX Γ Δ A B m m' n n' s r t l C :
+Lemma erasure_pair0_invX Γ Δ A B m m' n n' s r t l C :
   Γ ; Δ ⊢ Pair0 m n s ~ Pair0 m' n' s : C ->
   C ≃ Sig0 A B r ->
   Γ ⊢ Sig0 A B r : Sort t l ->
@@ -138,20 +138,20 @@ Proof with eauto.
   elim: ty A B m m' n n' s r t l e1 e2=>//{Γ Δ x y C}.
   { move=>Γ Δ A B m m' n t l ty1 tym ihm tyn A0 B0 m0 m0' n0 n'
       s r t0 l0[e1 e2 e3][e4 e5 e6]/sig0_inj[e7[e8 e9]]ty2; subst.
-    have[s[r0[l1[l2[ord[tyA0[tyB0/sort_inj[e1 e2]]]]]]]]:=sta_sig0_inv ty2. subst.
-    have tym0:Γ ; Δ ⊢ m ~ m' : A0 by apply: era_conv; eauto.
+    have[s[r0[l1[l2[ord[tyA0[tyB0/sort_inj[e1 e2]]]]]]]]:=logical_sig0_inv ty2. subst.
+    have tym0:Γ ; Δ ⊢ m ~ m' : A0 by apply: erasure_conv; eauto.
     repeat split...
-    apply: sta_conv.
-    apply: sta_conv_subst.
+    apply: logical_conv.
+    apply: logical_conv_subst.
     all: eauto.
-    apply: sta_esubst...
+    apply: logical_esubst...
     by autosubst. }
   { move=>Γ Δ A B m m' s l eq tym ihm tyB A0 B0 m0 m0' n n' s0 r t l0 e1 e2 eq' ty.
     apply: ihm...
     apply: conv_trans... }
 Qed.
 
-Lemma era_pair1_invX Γ Δ A B m m' n n' s r t l C :
+Lemma erasure_pair1_invX Γ Δ A B m m' n n' s r t l C :
   Γ ; Δ ⊢ Pair1 m n s ~ Pair1 m' n' s : C ->
   C ≃ Sig1 A B r ->
   Γ ⊢ Sig1 A B r : Sort t l ->
@@ -165,35 +165,35 @@ Proof with eauto.
   { move=>Γ Δ1 Δ2 Δ A B m m' n n' t l mrg ty1 tym ihm tyn ihn A0 B0
       m0 m0' n0 n0' s r t0 l0[e1 e2 e3][e4 e5 e6]/sig1_inj[e7[e8 e9]]ty2; subst.
     exists Δ1. exists Δ2.
-    have[s[r0[l1[l2[ord1[ord2[tyA0[tyB0/sort_inj[e1 e2]]]]]]]]]:=sta_sig1_inv ty2. subst.
-    have tym0:Γ ; Δ1 ⊢ m ~ m' : A0 by apply: era_conv; eauto.
+    have[s[r0[l1[l2[ord1[ord2[tyA0[tyB0/sort_inj[e1 e2]]]]]]]]]:=logical_sig1_inv ty2. subst.
+    have tym0:Γ ; Δ1 ⊢ m ~ m' : A0 by apply: erasure_conv; eauto.
     repeat split...
-    apply: era_conv.
-    apply: sta_conv_subst.
+    apply: erasure_conv.
+    apply: logical_conv_subst.
     all: eauto.
-    apply: sta_esubst...
+    apply: logical_esubst...
     by autosubst. }
   { move=>Γ Δ A B m m' s l eq tym ihm tyB A0 B0 m0 m0' n n' s0 r t l0 e1 e2 eq' ty.
     apply: ihm...
     apply: conv_trans... }
 Qed.
 
-Lemma era_pair0_inv Γ Δ A B m m' n n' s r :
+Lemma erasure_pair0_inv Γ Δ A B m m' n n' s r :
   Γ ; Δ ⊢ Pair0 m n s ~ Pair0 m' n' s : Sig0 A B r ->
   s = r /\ n' = Box /\ Γ ; Δ ⊢ m ~ m' : A /\ Γ ⊢ n : B.[m/].
 Proof with eauto.
   move=>ty.
-  have[t[lS tyS]]:=dyn_valid (era_dyn_type ty).
-  apply: era_pair0_invX...
+  have[t[lS tyS]]:=program_valid (erasure_program_type ty).
+  apply: erasure_pair0_invX...
 Qed.
 
-Lemma era_pair1_inv Γ Δ A B m m' n n' s r :
+Lemma erasure_pair1_inv Γ Δ A B m m' n n' s r :
   Γ ; Δ ⊢ Pair1 m n s ~ Pair1 m' n' s : Sig1 A B r ->
   exists Δ1 Δ2,
     Δ1 ∘ Δ2 => Δ /\ s = r /\
     Γ ; Δ1 ⊢ m ~ m' : A /\ Γ ; Δ2 ⊢ n ~ n' : B.[m/].
 Proof with eauto.
   move=>ty.
-  have[t[lS tyS]]:=dyn_valid (era_dyn_type ty).
-  apply: era_pair1_invX...
+  have[t[lS tyS]]:=program_valid (erasure_program_type ty).
+  apply: erasure_pair1_invX...
 Qed.
