coq/theories/heap_prg.v
@@ -1,14 +1,14 @@
 From mathcomp Require Import ssreflect ssrbool eqtype ssrnat seq.
 From Stdlib Require Import ssrfun Classical Utf8.
-Require Export AutosubstSsr ARS era_prog ptr_step ptr_sr.
+Require Export AutosubstSsr ARS erasure_prg heap_step heap_sr.
 
 Set Implicit Arguments.
 Unset Strict Implicit.
 Unset Printing Implicit Defensive.
 
-Lemma ptr_step_merge H1 H1' H2 H m n :
+Lemma heap_step_merge H1 H1' H2 H m n :
   H1 ; m ~>> H1' ; n -> H1 ∘ H2 => H -> exists H' n', H ; m ~>> H' ; n'.
-Proof with eauto using ptr_step, merge.
+Proof with eauto using heap_step, merge.
   move=>st. elim: st H2 H=>{H1 H1' m n}.
   { move=>H m s l h H2 H0 mrg; subst.
     have[l0 h0]:=hdomm_exist H0. case: s.
@@ -105,10 +105,10 @@ Proof with eauto.
   inv H8. exists l0. by exists l1.
 Qed.
 
-Theorem ptr_prog H x y z A :
+Theorem heap_prg H x y z A :
   H ; x ~ y ~ z : A -> wr_heap H ->
   (exists H' z', H ; z ~>> H' ; z') \/ (exists l, z = Ptr l).
-Proof with eauto using ptr_step.
+Proof with eauto using heap_step.
   move=>{H x y z A}[H x y z A].
   move e1:(nil)=>Γ. move e2:(nil)=>Δ er.
   elim: er H z e1 e2=>{Γ Δ x y A}.
@@ -124,39 +124,39 @@ Proof with eauto using ptr_step.
   { move=>Γ Δ A B m m' n s erm ihm tyn H z e1 e2 rs wr; subst. inv rs.
     { have[[H'[z' st]]|[l e]]:=ihm _ _ erefl erefl H4 wr.
       { left. exists H'. exists (App z' Box)... }
-      { subst. have vl':=wr_resolve_ptr wr H4.
-        have vl:=era_dyn_val erm vl'.
-        have[A0[m0 e]]:=dyn_pi0_canonical (era_dyn_type erm) (convR _ _) vl. subst.
-        have[m'0 e]:=era_lam0_canonical erm. subst.
+      { subst. have vl':=wr_resolve_heap wr H4.
+        have vl:=erasure_program_val erm vl'.
+        have[A0[m0 e]]:=program_pi0_canonical (erasure_program_type erm) (convR _ _) vl. subst.
+        have[m'0 e]:=erasure_lam0_canonical erm. subst.
         inv H4. inv H5.
         { left. exists H'. exists m1.[Box/]... }
-        { exfalso. apply: free_wr_ptr... } } }
+        { exfalso. apply: free_wr_heap... } } }
     { have[wr1 wr2]:=wr_merge_inv H5 wr.
       have//:=resolve_wr_box wr2 H9. }
     { inv H2.
-      { have vl:=wr_free_dyn_val H1 wr. inv vl. }
+      { have vl:=wr_free_program_val H1 wr. inv vl. }
       { have wr':=free_wr H1 wr.
         have[wr1 wr2]:=wr_merge_inv H7 wr'.
         have//:=resolve_wr_box wr2 H11. }
-      { exfalso. apply: free_wr_ptr... } } }
+      { exfalso. apply: free_wr_heap... } } }
   { move=>Γ Δ1 Δ2 Δ A B m m' n n' s mrg erm ihm ern ihn H z e1 e2 rs wr.
     subst; inv mrg. inv rs.
-    { have//:=era_box_form ern. }
+    { have//:=erasure_box_form ern. }
     { left. have[wr1 wr2]:=wr_merge_inv H5 wr.
       have[[H1'[m1 st1]]|[l1 e1]]:=ihm _ _ erefl erefl H8 wr1.
-      { have[H'[m0' st']]:=ptr_step_merge st1 H5.
+      { have[H'[m0' st']]:=heap_step_merge st1 H5.
         exists H'. exists (App m0' n0)... }
       { subst. have[[H2'[m2 st2]]|[l2 e2]]:=ihn _ _ erefl erefl H9 wr2.
-        { have[H'[m2' st']]:=ptr_step_merge st2 (hmrg_sym H5).
+        { have[H'[m2' st']]:=heap_step_merge st2 (hmrg_sym H5).
           exists H'. exists (App (Ptr l1) m2')... }
         { subst.
-          have vm':=wr_resolve_ptr wr1 H8.
-          have vm:=era_dyn_val erm vm'.
-          have[A0[m0 e]]:=dyn_pi1_canonical (era_dyn_type erm) (convR _ _) vm. subst.
-          have[m1 e]:=era_lam1_canonical erm. subst. inv H8. inv H7.
+          have vm':=wr_resolve_heap wr1 H8.
+          have vm:=erasure_program_val erm vm'.
+          have[A0[m0 e]]:=program_pi1_canonical (erasure_program_type erm) (convR _ _) vm. subst.
+          have[m1 e]:=erasure_lam1_canonical erm. subst. inv H8. inv H7.
           { have[H6[fr' mrg']]:=free_merge H4 H5.
             exists H6. exists m2.[Ptr l2/]... }
-          { exfalso. apply: free_wr_ptr... } } } }
+          { exfalso. apply: free_wr_heap... } } } }
     { right. exists l... } }
   { move=>Γ Δ A B m m' n t l0 tyS erm ihm tyn H z e1 e2 rs wr; subst. inv rs.
     { have[[H'[m1 st]]|[l e]]:=ihm _ _ erefl erefl H4 wr.
@@ -169,10 +169,10 @@ Proof with eauto using ptr_step.
     subst; inv mrg. inv rs.
     { left. have[wr1 wr2]:=wr_merge_inv H8 wr.
       have[[H1'[m1 st1]]|[l1 e1]]:=ihm _ _ erefl erefl H9 wr1.
-      { have[H'[m0' st']]:=ptr_step_merge st1 H8.
+      { have[H'[m0' st']]:=heap_step_merge st1 H8.
         exists H'. exists (Pair1 m0' n0 t)... }
       { subst. have[[H2'[m2 st2]]|[l2 e2]]:=ihn _ _ erefl erefl H10 wr2.
-        { have[H'[n0' st']]:=ptr_step_merge st2 (hmrg_sym H8).
+        { have[H'[n0' st']]:=heap_step_merge st2 (hmrg_sym H8).
           exists H'. exists (Pair1 (Ptr l1) n0' t)... }
         { subst. have[l3 h]:=hdomm_exist H.
           exists (setm H l3 (Pair1 (Ptr l1) (Ptr l2) t, t)).
@@ -182,33 +182,33 @@ Proof with eauto using ptr_step.
     subst; inv mrg. inv rs.
     { left. have[wr1 wr2]:=wr_merge_inv H5 wr.
       have[[H1'[m1 st]]|[l e]]:=ihm _ _ erefl erefl H8 wr1.
-      { have[H'[m0' st']]:=ptr_step_merge st H5.
+      { have[H'[m0' st']]:=heap_step_merge st H5.
         exists H'. exists (LetIn Box m0' n0)... }
       { subst.
-        have vm':=wr_resolve_ptr wr1 H8.
-        have vm:=era_dyn_val erm vm'.
-        have[m1[m2 e]]:=dyn_sig0_canonical (era_dyn_type erm) (convR _ _) vm. subst.
-        have[m0 e]:=era_pair0_canonical erm. subst. inv H8. inv H7.
+        have vm':=wr_resolve_heap wr1 H8.
+        have vm:=erasure_program_val erm vm'.
+        have[m1[m2 e]]:=program_sig0_canonical (erasure_program_type erm) (convR _ _) vm. subst.
+        have[m0 e]:=erasure_pair0_canonical erm. subst. inv H8. inv H7.
         { have[H6[fr' mrg']]:=free_merge H4 H5.
           have[lm[e _]]:=free_pair0_canonical wr fr'. subst.
           exists H6. exists (n0.[Box,Ptr lm/])... }
-        { exfalso. apply: free_wr_ptr... } } }
+        { exfalso. apply: free_wr_heap... } } }
     { right. exists l... } }
   { move=>Γ Δ1 Δ2 Δ A B C m m' n n' s r1 r2 t l0 mrg tyC erm ihm ern _ H z e1 e2 rs wr.
     subst; inv mrg. inv rs.
     { left. have[wr1 wr2]:=wr_merge_inv H5 wr.
       have[[H1'[m1 st]]|[l e]]:=ihm _ _ erefl erefl H8 wr1.
-      { have[H'[m0' st']]:=ptr_step_merge st H5.
+      { have[H'[m0' st']]:=heap_step_merge st H5.
         exists H'. exists (LetIn Box m0' n0)... }
       { subst.
-        have vm':=wr_resolve_ptr wr1 H8.
-        have vm:=era_dyn_val erm vm'.
-        have[m1[m2 e]]:=dyn_sig1_canonical (era_dyn_type erm) (convR _ _) vm. subst.
-        have[m1'[m2' e]]:=era_pair1_canonical erm. subst. inv H8. inv H7.
+        have vm':=wr_resolve_heap wr1 H8.
+        have vm:=erasure_program_val erm vm'.
+        have[m1[m2 e]]:=program_sig1_canonical (erasure_program_type erm) (convR _ _) vm. subst.
+        have[m1'[m2' e]]:=erasure_pair1_canonical erm. subst. inv H8. inv H7.
         { have[H6[fr' mrg']]:=free_merge H4 H5.
           have[lm[ln[e1 e2]]]:=free_pair1_canonical wr fr'. subst.
           exists H6. exists (n0.[Ptr ln,Ptr lm/])... }
-        { exfalso. apply: free_wr_ptr... } } }
+        { exfalso. apply: free_wr_heap... } } }
     { right. exists l... } }
   { move=>Γ Δ wf k H z e1 e2 rs wr; subst. inv rs.
     { left. have[l h]:=hdomm_exist H. exists (setm H l (TT, U)). exists (Ptr l)... }
@@ -221,18 +221,18 @@ Proof with eauto using ptr_step.
     subst; inv mrg. inv rs.
     { left. have[wr1 wr2]:=wr_merge_inv H6 wr.
       have[[H1'[m1 st]]|[l0 e]]:=ihm _ _ erefl erefl H9 wr1.
-      { have[H'[m0' st']]:=ptr_step_merge st H6.
+      { have[H'[m0' st']]:=heap_step_merge st H6.
         exists H'. exists (Ifte Box m0' n0 n3)... }
       { subst.
-        have vm':=wr_resolve_ptr wr1 H9.
-        have vm:=era_dyn_val erm vm'.
-        have[e|e]:=dyn_bool_canonical (era_dyn_type erm) (convR _ _) vm.
-        { subst. have e:=era_tt_canonical erm. subst. inv H9. inv H7.
+        have vm':=wr_resolve_heap wr1 H9.
+        have vm:=erasure_program_val erm vm'.
+        have[e|e]:=program_bool_canonical (erasure_program_type erm) (convR _ _) vm.
+        { subst. have e:=erasure_tt_canonical erm. subst. inv H9. inv H7.
           have[H7[fr' mrg']]:=free_merge H4 H6.
-          exists H7. exists n0... exfalso. apply: free_wr_ptr... }
-        { subst. have e:=era_ff_canonical erm. subst. inv H9. inv H7.
+          exists H7. exists n0... exfalso. apply: free_wr_heap... }
+        { subst. have e:=erasure_ff_canonical erm. subst. inv H9. inv H7.
           have[H7[fr' mrg']]:=free_merge H4 H6.
-          exists H7. exists n3... exfalso. apply: free_wr_ptr... } } }
+          exists H7. exists n3... exfalso. apply: free_wr_heap... } } }
     { right. exists l0... } }
   { move=>Γ Δ A B x x' P m n s l0 tyB erx ihx tyP H z e1 e2 rs wr; subst. inv rs.
     { left. exists H. exists m0... }
