coq/theories/heap_sr.v
@@ -1,18 +1,18 @@
 From mathcomp Require Import ssreflect ssrbool eqtype ssrnat seq.
 From Stdlib Require Import ssrfun Classical Utf8.
-Require Export AutosubstSsr ARS era_sr ptr_step ptr_subst.
+Require Export AutosubstSsr ARS erasure_sr heap_step heap_subst.
 
 Set Implicit Arguments.
 Unset Strict Implicit.
 Unset Printing Implicit Defensive.
 
-Lemma ptr_srX H1 H2 H H' x y z z' A :
+Lemma heap_srX H1 H2 H H' x y z z' A :
   H1 ; x ~ y ~ z : A -> wr_heap H ->
   H1 ∘ H2 => H -> H ; z ~>> H' ; z' ->
   exists H1' H2' x' y',
     H1' ; x' ~ y' ~ z' : A /\ wr_heap H' /\
     pad H2 H2' /\ H1' ∘ H2' => H' /\ x ~>>* x' /\ y ~>>* y'.
-Proof with eauto 7 using era_type, resolve, dyn_step, key, merge, hmrg_setmU, hmrg_setmL, pad_refl.
+Proof with eauto 7 using erasure_type, resolve, program_step, key, merge, hmrg_setmU, hmrg_setmL, pad_refl.
   move=>{H1 x y z A}[H1 x y z A].
   move e1:(nil)=>Γ. move e2:(nil)=>Δ er.
   elim: er H1 H2 H H' z z' e1 e2=>{Γ Δ x y A}.
@@ -100,17 +100,17 @@ Proof with eauto 7 using era_type, resolve, dyn_step, key, merge, hmrg_setmU, hm
       exists H1'. exists H2'. exists (App x' n). exists (App y' Box).
       repeat split...
       { apply: (star_hom (App^~ n)) rd1=>x y.
-        apply: dyn_step_appL. }
+        apply: program_step_appL. }
       { apply: (star_hom (App^~ Box)) rd2=>x y.
-        apply: dyn_step_appL. } }
+        apply: program_step_appL. } }
     { inv H9. }
     { have[H1'[mrg' rs]]:=resolve_free H9 H6 mrg. inv rs.
-      have[A0[n0 e]]:=era_lam0_form erm. subst.
+      have[A0[n0 e]]:=erasure_lam0_form erm. subst.
       exists H1'. exists H2. exists (n0.[n/]). exists (m'0.[Box/]).
       repeat split...
-      { have[ern0 _]:=era_lam0_inv erm.
-        apply: era_esubst0... }
-      { have[ern _]:=era_lam0_inv erm.
+      { have[ern0 _]:=erasure_lam0_inv erm.
+        apply: erasure_esubst0... }
+      { have[ern _]:=erasure_lam0_inv erm.
         have wr':=free_wr H9 wr.
         have[wr1 wr2]:=wr_merge_inv mrg' wr'.
         have[Hx[k mrgx]]:=hsplit_self H1'.
@@ -135,9 +135,9 @@ Proof with eauto 7 using era_type, resolve, dyn_step, key, merge, hmrg_setmU, hm
       have//:=resolve_wr_box wr4 H11. } }
   { move=>Γ Δ1 Δ2 Δ A B m m' n n' s mrg1 erm ihm ern ihn H1 H2 H H' z z' e1 e2 rs wr mrg2 st; subst.
     inv mrg1. inv rs; inv st.
-    { have//:=era_box_form ern. }
-    { have//:=era_box_form ern. }
-    { have//:=era_box_form ern. }
+    { have//:=erasure_box_form ern. }
+    { have//:=erasure_box_form ern. }
+    { have//:=erasure_box_form ern. }
     { have[wr1 wr2]:=wr_merge_inv mrg2 wr.
       have[H4[mrg3 mrg4]]:=hmrg_splitR mrg2 H7.
       have[H1'[H2'[x'[y'[wrx[wr'[pd[mrg5[rd1 rd2]]]]]]]]]:=
@@ -152,9 +152,9 @@ Proof with eauto 7 using era_type, resolve, dyn_step, key, merge, hmrg_setmU, hm
         apply: H8.
         apply: resolve_pad... }
       { apply: (star_hom (App^~ n)) rd1=>x y.
-        apply: dyn_step_appL. }
+        apply: program_step_appL. }
       { apply: (star_hom (App^~ n')) rd2=>x y.
-        apply: dyn_step_appL. } }
+        apply: program_step_appL. } }
     { have[H4[mrg3 mrg4]]:=hmrg_splitL mrg2 H7.
       have[H1'[H2'[x'[y'[wrx[wr'[pd[mrg5[rd1 rd2]]]]]]]]]:=
         ihn _ _ _ _ _ _ erefl erefl H11 wr (hmrg_sym mrg4) H13.
@@ -163,47 +163,47 @@ Proof with eauto 7 using era_type, resolve, dyn_step, key, merge, hmrg_setmU, hm
       inv wrx.
       exists Hx. exists H2p. exists (App m x'). exists (App m' y').
       repeat split...
-      { have[t[lP tyP]]:=dyn_valid (era_dyn_type erm).
-        have[r[l1[l2[tyB/sort_inj[e1 e2]]]]]:=sta_pi1_inv tyP. subst.
-        have tyn:=dyn_sta_type (era_dyn_type ern).
-        have//=tyBn:=sta_subst tyB tyn.
-        apply: era_conv.
-        apply: sta_conv_beta.
+      { have[t[lP tyP]]:=program_valid (erasure_program_type erm).
+        have[r[l1[l2[tyB/sort_inj[e1 e2]]]]]:=logical_pi1_inv tyP. subst.
+        have tyn:=program_logical_type (erasure_program_type ern).
+        have//=tyBn:=logical_subst tyB tyn.
+        apply: erasure_conv.
+        apply: logical_conv_beta.
         apply: conv_sym.
         apply: star_conv.
-        apply: dyn_sta_red...
+        apply: program_logical_red...
         econstructor...
         apply: tyBn. }
       { econstructor...
         apply: resolve_pad... }
       { apply: (star_hom (App m)) rd1=>x y.
-        apply: dyn_step_appR. }
+        apply: program_step_appR. }
       { apply: (star_hom (App m')) rd2=>x y.
-        apply: dyn_step_appR. } }
+        apply: program_step_appR. } }
     { have[Hx[mrg3 mrg4]]:=hmrg_splitR mrg2 H7.
       have[Hy[mrg5 rs]]:=resolve_free H13 H10 (hmrg_sym mrg4). inv rs.
-      have[A0[n1 e]]:=era_lam0_form erm. subst.
-      exfalso. apply: sta_lam0_pi1_false... }
+      have[A0[n1 e]]:=erasure_lam0_form erm. subst.
+      exfalso. apply: logical_lam0_pi1_false... }
     { have[H4[mrg3 mrg4]]:=hmrg_splitR mrg2 H7.
       have[H5[mrg rs]]:=resolve_free H13 H10 (hmrg_sym mrg4). inv rs.
       have[Hx[mrg5 mrg6]]:=hmrg_splitL (hmrg_sym mrg) mrg3.
-      have[A0[n0 e]]:=era_lam1_form erm. subst.
-      have[r[ern0 _]]:=era_lam1_inv erm.
+      have[A0[n0 e]]:=erasure_lam1_form erm. subst.
+      have[r[ern0 _]]:=erasure_lam1_inv erm.
       have wr':=free_wr H13 wr.
       have[wr1 wr2]:=wr_merge_inv mrg wr'.
       have[wr3 wr4]:=wr_merge_inv mrg3 wr2.
       have[H3'[k mrg']]:=hsplit_self H3.
       have[_ wr3']:=wr_merge_inv mrg' wr3.
-      have vl':=wr_resolve_ptr wr3 H11.
-      have vl:=era_dyn_val ern vl'.
+      have vl':=wr_resolve_heap wr3 H11.
+      have vl:=erasure_program_val ern vl'.
       exists Hx. exists H2. exists n0.[n/]. exists m'0.[n'/].
       repeat split...
-      { apply: era_subst1.
+      { apply: erasure_subst1.
         apply: key_nil.
         apply: merge_nil.
         apply: ern0.
         apply: ern. }
-      { have wf:=dyn_type_wf (era_dyn_type ern0). inv wf.
+      { have wf:=program_type_wf (erasure_program_type ern0). inv wf.
         have k1:=resolution (Ptr_well_resolved ern H11) H17 vl' wr3.
         destruct r.
         { apply: resolve_subst.
@@ -223,8 +223,8 @@ Proof with eauto 7 using era_type, resolve, dyn_step, key, merge, hmrg_setmU, hm
           apply: hmrg_sym...
           all: eauto.
           constructor... } }
-      { apply: star1. apply: dyn_step_beta1... }
-      { apply: star1. apply: dyn_step_beta1... } } }
+      { apply: star1. apply: program_step_beta1... }
+      { apply: star1. apply: program_step_beta1... } } }
   { move=>Γ Δ A B m m' n t l tyS erm ihm tyn H1 H2 H H' z z' e1 e2 rs wr mrg st; subst.
     have[wr1 wr2]:=wr_merge_inv mrg wr.
     inv rs; inv st.
@@ -232,20 +232,20 @@ Proof with eauto 7 using era_type, resolve, dyn_step, key, merge, hmrg_setmU, hm
       inv wrx.
       exists H1'. exists H2'. exists (Pair0 x' n t). exists (Pair0 y' Box t).
       rsplit...
-      { have[s[r[l1[l2[ord[tyA[tyB _]]]]]]]:=sta_sig0_inv tyS.
-        have tyx:=dyn_sta_type (dyn_rd (era_dyn_type erm) rd1).
-        have//=tyBx:=sta_subst tyB tyx.
+      { have[s[r[l1[l2[ord[tyA[tyB _]]]]]]]:=logical_sig0_inv tyS.
+        have tyx:=program_logical_type (program_rd (erasure_program_type erm) rd1).
+        have//=tyBx:=logical_subst tyB tyx.
         econstructor...
-        apply: sta_conv.
-        apply: sta_conv_beta.
+        apply: logical_conv.
+        apply: logical_conv_beta.
         apply: star_conv.
-        apply: (dyn_sta_red (dyn_sta_type (era_dyn_type erm)))...
+        apply: (program_logical_red (program_logical_type (erasure_program_type erm)))...
         apply: tyn.
         apply: tyBx. }
       { apply: (star_hom ((Pair0^~ n)^~ t)) rd1=>x y.
-        apply: dyn_step_pair0L. }
+        apply: program_step_pair0L. }
       { apply: (star_hom ((Pair0^~ Box)^~ t)) rd2=>x y.
-        apply: dyn_step_pair0L. } }
+        apply: program_step_pair0L. } }
     { destruct t.
       { exists (setm H1 l0 (Pair0 (Ptr lm) Box U, U)).
         exists (setm H2 l0 (Pair0 (Ptr lm) Box U, U)).
@@ -278,7 +278,7 @@ Proof with eauto 7 using era_type, resolve, dyn_step, key, merge, hmrg_setmU, hm
           move=>x. have:=wr1 x. rewrite setmE. by case: eqP.
           exact: wr2. } } } }
   { move=>Γ Δ1 Δ2 Δ A B m m' n n' t l mrg1 tyS erm ihm ern ihn H1 H2 H H' z z' e1 e2 rs wr mrg2 st; subst.
-    have[s[r[l1[l2[ord1[ord2[tyA[tyB _]]]]]]]]:=sta_sig1_inv tyS. inv mrg1.
+    have[s[r[l1[l2[ord1[ord2[tyA[tyB _]]]]]]]]:=logical_sig1_inv tyS. inv mrg1.
     have[wr1 wr2]:=wr_merge_inv mrg2 wr.
     inv rs; inv st.
     { have[H4[mrg3 mrg4]]:=hmrg_splitR mrg2 H10.
@@ -288,13 +288,13 @@ Proof with eauto 7 using era_type, resolve, dyn_step, key, merge, hmrg_setmU, hm
       have[Hx[mrp1 mrp2]]:=hmrg_splitL (hmrg_sym mrg') mrp.
       exists Hx. exists H2p. exists (Pair1 x' n t). exists (Pair1 y' n' t).
       repeat split...
-      { have tyx:=dyn_sta_type (dyn_rd (era_dyn_type erm) rd1).
-        have//=tyBx:=sta_subst tyB tyx.
+      { have tyx:=program_logical_type (program_rd (erasure_program_type erm) rd1).
+        have//=tyBx:=logical_subst tyB tyx.
         econstructor...
-        apply: era_conv.
-        apply: sta_conv_beta.
+        apply: erasure_conv.
+        apply: logical_conv_beta.
         apply: star_conv.
-        apply: (dyn_sta_red (dyn_sta_type (era_dyn_type erm)))...
+        apply: (program_logical_red (program_logical_type (erasure_program_type erm)))...
         apply: ern.
         apply: tyBx. }
       { econstructor.
@@ -302,9 +302,9 @@ Proof with eauto 7 using era_type, resolve, dyn_step, key, merge, hmrg_setmU, hm
         apply: H7.
         apply: resolve_pad... }
       { apply: (star_hom ((Pair1^~ n)^~ t)) rd1=>x y.
-        apply: dyn_step_pair1L. }
+        apply: program_step_pair1L. }
       { apply: (star_hom ((Pair1^~ n')^~ t)) rd2=>x y.
-        apply: dyn_step_pair1L. } }
+        apply: program_step_pair1L. } }
     { have[H4[mrg3 mrg4]]:=hmrg_splitL mrg2 H10.
       have[H1'[H2'[x'[y'[wrx[wr'[pd[mrg'[rd1 rd2]]]]]]]]]:=
         ihn _ _ _ _ _ _ erefl erefl H12 wr (hmrg_sym mrg4) H14. inv wrx.
@@ -315,9 +315,9 @@ Proof with eauto 7 using era_type, resolve, dyn_step, key, merge, hmrg_setmU, hm
       { econstructor...
         apply: resolve_pad... }
       { apply: (star_hom (Pair1 m^~ t)) rd1=>x y.
-        apply: dyn_step_pair1R. }
+        apply: program_step_pair1R. }
       { apply: (star_hom (Pair1 m'^~ t)) rd2=>x y.
-        apply: dyn_step_pair1R. } }
+        apply: program_step_pair1R. } }
     { destruct t.
       { exists (setm H1 l0 (Pair1 (Ptr lm) (Ptr ln) U, U)).
         exists (setm H2 l0 (Pair1 (Ptr lm) (Ptr ln) U, U)).
@@ -359,33 +359,33 @@ Proof with eauto 7 using era_type, resolve, dyn_step, key, merge, hmrg_setmU, hm
       have[Hx[mrp1 mrp2]]:=hmrg_splitL (hmrg_sym mrg') mrp.
       exists Hx. exists H2p. exists (LetIn C x' n). exists (LetIn Box y' n').
       repeat split...
-      { apply: era_conv.
-        apply: sta_conv_beta.
+      { apply: erasure_conv.
+        apply: logical_conv_beta.
         apply: conv_sym.
         apply: star_conv.
-        apply: dyn_sta_red...
-        apply: era_letin0...
-        apply: sta_esubst...
+        apply: program_logical_red...
+        apply: erasure_letin0...
+        apply: logical_esubst...
         autosubst. }
       { econstructor.
         apply: hmrg_sym...
         apply: H8.
         apply: resolve_pad... }
       { apply: (star_hom (LetIn C^~ n)) rd1=>x y.
-        apply: dyn_step_letinL. }
+        apply: program_step_letinL. }
       { apply: (star_hom (LetIn Box^~ n')) rd2=>x y.
-        apply: dyn_step_letinL. } }
+        apply: program_step_letinL. } }
     { have[H4[mrg3 mrg4]]:=hmrg_splitR mrg2 H7.
       have[H1'[mrg' rs]]:=resolve_free H13 H10 (hmrg_sym mrg4). inv rs.
       have[Hx[mrg5 mrg6]]:=hmrg_splitL (hmrg_sym mrg') mrg3.
-      have[m1[m2 e]]:=era_pair0_form erm. subst.
-      have[e[_[erm1 tym2]]]:=era_pair0_inv erm. subst.
+      have[m1[m2 e]]:=erasure_pair0_form erm. subst.
+      have[e[_[erm1 tym2]]]:=erasure_pair0_inv erm. subst.
       have wr':=free_wr H13 wr.
       have[wr1 wr2]:=wr_merge_inv mrg2 wr.
       have[wr3 wr4]:=wr_merge_inv H7 wr1.
       have[wr5 wr6]:=wr_merge_inv mrg' wr'.
-      have vl:=wr_resolve_ptr wr5 H15.
-      have wf:=dyn_type_wf (era_dyn_type ern). inv wf.  inv H9.
+      have vl:=wr_resolve_heap wr5 H15.
+      have wf:=program_type_wf (erasure_program_type ern). inv wf.  inv H9.
       have k1:=resolution (Ptr_well_resolved erm1 H15) H17 vl wr5.
       have[H2'[k mrg2']]:=hsplit_self H1'.
       have[_ wr7]:=wr_merge_inv mrg2' wr5.
@@ -393,7 +393,7 @@ Proof with eauto 7 using era_type, resolve, dyn_step, key, merge, hmrg_setmU, hm
       repeat split...
       { replace C.[Pair0 m1 m2 t/] with
           C.[Pair0 (Var 1) (Var 0) t .: ren (+2)].[m2,m1/] by autosubst.
-        apply: era_substitution.
+        apply: erasure_substitution.
         apply: ern.
         constructor.
         econstructor.
@@ -416,14 +416,14 @@ Proof with eauto 7 using era_type, resolve, dyn_step, key, merge, hmrg_setmU, hm
       { apply: star1.
         constructor.
         constructor.
-        apply: era_dyn_val... }
+        apply: erasure_program_val... }
       { apply: star1.
         constructor.
         constructor... } }
     { have[H4[mrg3 mrg4]]:=hmrg_splitR mrg2 H7.
       have[H1'[mrg' rs]]:=resolve_free H13 H10 (hmrg_sym mrg4). inv rs.
-      have[m1[m2 e]]:=era_pair1_form erm. subst.
-      exfalso. apply: sta_pair1_sig0_false... } }
+      have[m1[m2 e]]:=erasure_pair1_form erm. subst.
+      exfalso. apply: logical_pair1_sig0_false... } }
   { move=>Γ Δ1 Δ2 Δ A B C m m' n n' s r1 r2 t l mrg1 tyC
       erm ihm ern _ H1 H2 H H' z z' e1 e2 rs wr mrg2 st; subst.
     inv mrg1. inv rs; inv st.
@@ -434,41 +434,41 @@ Proof with eauto 7 using era_type, resolve, dyn_step, key, merge, hmrg_setmU, hm
       have[Hx[mrp1 mrp2]]:=hmrg_splitL (hmrg_sym mrg') mrp.
       exists Hx. exists H2p. exists (LetIn C x' n). exists (LetIn Box y' n').
       repeat split...
-      { apply: era_conv.
-        apply: sta_conv_beta.
+      { apply: erasure_conv.
+        apply: logical_conv_beta.
         apply: conv_sym.
         apply: star_conv.
-        apply: dyn_sta_red...
-        apply: era_letin1...
-        apply: sta_esubst...
+        apply: program_logical_red...
+        apply: erasure_letin1...
+        apply: logical_esubst...
         autosubst. }
       { econstructor.
         apply: hmrg_sym...
         apply: H8.
         apply: resolve_pad... }
       { apply: (star_hom (LetIn C^~ n)) rd1=>x y.
-        apply: dyn_step_letinL. }
+        apply: program_step_letinL. }
       { apply: (star_hom (LetIn Box^~ n')) rd2=>x y.
-        apply: dyn_step_letinL. } }
+        apply: program_step_letinL. } }
     { have[H4[mrg3 mrg4]]:=hmrg_splitR mrg2 H7.
       have[H1'[mrg' rs]]:=resolve_free H13 H10 (hmrg_sym mrg4). inv rs.
-      have[m1[m2 e]]:=era_pair0_form erm. subst.
-      exfalso. apply: sta_pair0_sig1_false... }
+      have[m1[m2 e]]:=erasure_pair0_form erm. subst.
+      exfalso. apply: logical_pair0_sig1_false... }
     { have[H4[mrg3 mrg4]]:=hmrg_splitR mrg2 H7.
       have[H1'[mrg' rs]]:=resolve_free H13 H10 (hmrg_sym mrg4). inv rs.
       have[Hx[mrg5 mrg6]]:=hmrg_splitL (hmrg_sym mrg') mrg3.
-      have[m1[m2 e]]:=era_pair1_form erm. subst.
-      have[Δ1[Δ2[mrg[e[erm1 erm2]]]]]:=era_pair1_inv erm. inv mrg; subst.
+      have[m1[m2 e]]:=erasure_pair1_form erm. subst.
+      have[Δ1[Δ2[mrg[e[erm1 erm2]]]]]:=erasure_pair1_inv erm. inv mrg; subst.
       have wr':=free_wr H13 wr.
       have[wr1 wr2]:=wr_merge_inv mrg2 wr.
       have[wr3 wr4]:=wr_merge_inv H7 wr1.
       have[wr5 wr6]:=wr_merge_inv mrg' wr'.
       have[wr7 wr8]:=wr_merge_inv H16 wr5.
-      have vm:=wr_resolve_ptr wr7 H18.
-      have vn:=wr_resolve_ptr wr8 H19.
-      have wf:=dyn_type_wf (era_dyn_type ern). inv wf.  inv H14.
+      have vm:=wr_resolve_heap wr7 H18.
+      have vn:=wr_resolve_heap wr8 H19.
+      have wf:=program_type_wf (erasure_program_type ern). inv wf.  inv H14.
       have k1:=resolution (Ptr_well_resolved erm1 H18) H21 vm wr7.
-      have//=tyBm1:=sta_subst H17 (dyn_sta_type (era_dyn_type erm1)).
+      have//=tyBm1:=logical_subst H17 (program_logical_type (erasure_program_type erm1)).
       have k2:=resolution (Ptr_well_resolved erm2 H19) tyBm1 vn wr8.
       have[H5'[k5 mrg5']]:=hsplit_self H5.
       have[H6'[k6 mrg6']]:=hsplit_self H6.
@@ -478,7 +478,7 @@ Proof with eauto 7 using era_type, resolve, dyn_step, key, merge, hmrg_setmU, hm
       repeat split...
       { replace C.[Pair1 m1 m2 t/] with
           C.[Pair1 (Var 1) (Var 0) t .: ren (+2)].[m2,m1/] by autosubst.
-        apply: era_substitution.
+        apply: erasure_substitution.
         apply: ern.
         econstructor. apply: key_nil.
         constructor.
@@ -513,8 +513,8 @@ Proof with eauto 7 using era_type, resolve, dyn_step, key, merge, hmrg_setmU, hm
       { apply: star1.
         constructor.
         constructor.
-        apply: era_dyn_val...
-        apply: era_dyn_val... }
+        apply: erasure_program_val...
+        apply: erasure_program_val... }
       { apply: star1.
         constructor.
         constructor... } } }
@@ -554,13 +554,13 @@ Proof with eauto 7 using era_type, resolve, dyn_step, key, merge, hmrg_setmU, hm
       have[Hx[mrp1 mrp2]]:=hmrg_splitL (hmrg_sym mrg') mrp.
       exists Hx. exists H2p. exists (Ifte A x' n1 n2). exists (Ifte Box y' n1' n2').
       repeat split...
-      { apply: era_conv.
-        apply: sta_conv_beta.
+      { apply: erasure_conv.
+        apply: logical_conv_beta.
         apply: conv_sym.
         apply: star_conv.
-        apply: dyn_sta_red...
-        apply: era_ifte...
-        apply: sta_esubst...
+        apply: program_logical_red...
+        apply: erasure_ifte...
+        apply: logical_esubst...
         autosubst. }
       { econstructor.
         apply: hmrg_sym...
@@ -568,13 +568,13 @@ Proof with eauto 7 using era_type, resolve, dyn_step, key, merge, hmrg_setmU, hm
         apply: resolve_pad...
         apply: resolve_pad... }
       { apply: (star_hom ((Ifte A^~ n1)^~ n2)) rd1=>x y.
-        apply: dyn_step_ifteM. }
+        apply: program_step_ifteM. }
       { apply: (star_hom ((Ifte Box^~ n1')^~ n2')) rd2=>x y.
-        apply: dyn_step_ifteM. } }
+        apply: program_step_ifteM. } }
     { have[H4[mrg3 mrg4]]:=hmrg_splitR mrg2 H8.
       have[H1'[mrg' rs]]:=resolve_free H15 H11 (hmrg_sym mrg4). inv rs.
       have[Hx[mrg5 mrg6]]:=hmrg_splitL (hmrg_sym mrg') mrg3.
-      have e:=era_tt_form erm. subst.
+      have e:=erasure_tt_form erm. subst.
       have e:=hmrg_pureR mrg5 H6. subst.
       have wr':=free_wr H15 wr.
       exists H3. exists H2. exists n1. exists n1'.
@@ -584,7 +584,7 @@ Proof with eauto 7 using era_type, resolve, dyn_step, key, merge, hmrg_setmU, hm
     { have[H4[mrg3 mrg4]]:=hmrg_splitR mrg2 H8.
       have[H1'[mrg' rs]]:=resolve_free H15 H11 (hmrg_sym mrg4). inv rs.
       have[Hx[mrg5 mrg6]]:=hmrg_splitL (hmrg_sym mrg') mrg3.
-      have e:=era_ff_form erm. subst.
+      have e:=erasure_ff_form erm. subst.
       have e:=hmrg_pureR mrg5 H6. subst.
       have wr':=free_wr H15 wr.
       exists H3. exists H2. exists n2. exists n2'.
@@ -595,30 +595,30 @@ Proof with eauto 7 using era_type, resolve, dyn_step, key, merge, hmrg_setmU, hm
     inv rs; inv st.
     exists H1. exists H2. exists x. exists x'.
     repeat split...
-    { have[P0[rdP vlP]]:=sta_vn tyP.
-      have tyP0:=sta_rd tyP rdP.
-      have[n0 e]:=sta_id_canonical tyP0 (convR _ _) vlP. subst.
-      have tyr:=sta_rd tyP rdP.
-      have[r[lI tyI]]:=sta_valid tyP.
-      have[l0[tym[tyn/sort_inj[e1 e2]]]]:=sta_id_inv tyI. subst.
-      have[tym0[eq1 eq2]]:=sta_refl_inv tyr.
+    { have[P0[rdP vlP]]:=logical_vn tyP.
+      have tyP0:=logical_rd tyP rdP.
+      have[n0 e]:=logical_id_canonical tyP0 (convR _ _) vlP. subst.
+      have tyr:=logical_rd tyP rdP.
+      have[r[lI tyI]]:=logical_valid tyP.
+      have[l0[tym[tyn/sort_inj[e1 e2]]]]:=logical_id_inv tyI. subst.
+      have[tym0[eq1 eq2]]:=logical_refl_inv tyr.
       have sc:sconv (Refl m .: m .: ids) (P .: n .: ids).
       { move=>[|[|]]//=.
-        apply: conv_trans. apply: sta_conv_refl. apply: conv_sym...
+        apply: conv_trans. apply: logical_conv_refl. apply: conv_sym...
         apply: conv_sym. apply: star_conv...
         apply: conv_trans. apply: conv_sym... eauto. }
       have wkB:nil ⊢ B.[P,n/] : Sort s l.
       { replace (Sort s l) with (Sort s l).[P,n/] by eauto.
-        apply: sta_substitution...
+        apply: logical_substitution...
         repeat constructor...
         all: asimpl... }
-      apply: era_conv.
-      apply: sta_conv_compat sc.
+      apply: erasure_conv.
+      apply: logical_conv_compat sc.
       all: eauto. }
     { apply: star1.
-      apply: dyn_step_rwE. }
+      apply: program_step_rwE. }
     { apply: star1.
-      apply: dyn_step_rwE. } }
+      apply: program_step_rwE. } }
   { move=>Γ Δ A B m m' s l eq erm ihm tyB H1 H2 H H' z z' e1 e2 rs wr mrg st; subst.
     have[H1'[H2'[x'[y'[wrx[wr'[pd[mrg'[rd1 rd2]]]]]]]]]:=
       ihm _ _ _ _ _ _ erefl erefl rs wr mrg st. inv wrx.
@@ -626,14 +626,14 @@ Proof with eauto 7 using era_type, resolve, dyn_step, key, merge, hmrg_setmU, hm
     repeat split... }
 Qed.
 
-Theorem ptr_sr H H' x y z z' A :
+Theorem heap_sr H H' x y z z' A :
   H ; x ~ y ~ z : A -> wr_heap H ->
   H ; z ~>> H' ; z' ->
   exists x' y', H' ; x' ~ y' ~ z' : A /\ wr_heap H' /\ x ~>>* x' /\ y ~>>* y'.
 Proof with eauto.
   move=>wrx wr st.
   have[H0[k mrg]]:=hsplit_self H.
-  have[H1'[H2'[x'[y'[wrx'[wr'[pd[mrg'[rd1 rd2]]]]]]]]]:=ptr_srX wrx wr mrg st.
+  have[H1'[H2'[x'[y'[wrx'[wr'[pd[mrg'[rd1 rd2]]]]]]]]]:=heap_srX wrx wr mrg st.
   have k':=pad_key pd k.
   have e:=hmrg_pureR mrg' k'. subst.
   exists x'. exists y'...
