coq/theories/logical_prg.v
@@ -1,22 +1,22 @@
 From mathcomp Require Import ssreflect ssrbool eqtype ssrnat seq.
 From Stdlib Require Import ssrfun Classical Utf8.
-Require Export AutosubstSsr ARS sta_sr.
+Require Export AutosubstSsr ARS logical_sr.
 
 Set Implicit Arguments.
 Unset Strict Implicit.
 Unset Printing Implicit Defensive.
 
-Ltac inv_sta_val :=
+Ltac inv_logical_val :=
   match goal with
-  | [ H : sta_val _ |- _ ] => inv H
+  | [ H : logical_val _ |- _ ] => inv H
   end.
 
-Lemma sta_pi0_canonical m A B C s :
-  nil ⊢ m : C -> C ≃ Pi0 A B s -> sta_val m ->
+Lemma logical_pi0_canonical m A B C s :
+  nil ⊢ m : C -> C ≃ Pi0 A B s -> logical_val m ->
   exists A n, m = Lam0 A n s.
 Proof with eauto.
   move e:(nil)=>Γ ty. elim: ty e A B s=>{Γ m C}.
-  all: try solve[intros; exfalso; (solve_conv||inv_sta_val)].
+  all: try solve[intros; exfalso; (solve_conv||inv_logical_val)].
   { move=>Γ x A wf shs e A0 B s eq vl. subst. inv shs. }
   { move=>Γ A B m s tym ihm e1 A0 B0 s0/pi0_inj[eqA[eqB e2]] vl. subst.
     exists A. exists m... }
@@ -25,12 +25,12 @@ Proof with eauto.
     apply: conv_trans... }
 Qed.
 
-Lemma sta_pi1_canonical m A B C s :
-  nil ⊢ m : C -> C ≃ Pi1 A B s -> sta_val m ->
+Lemma logical_pi1_canonical m A B C s :
+  nil ⊢ m : C -> C ≃ Pi1 A B s -> logical_val m ->
   exists A n, m = Lam1 A n s.
 Proof with eauto.
   move e:(nil)=>Γ ty. elim: ty e A B s=>{Γ m C}.
-  all: try solve[intros; exfalso; (solve_conv||inv_sta_val)].
+  all: try solve[intros; exfalso; (solve_conv||inv_logical_val)].
   { move=>Γ x A wf shs e. subst. inv shs. }
   { move=>Γ A B m s tym ihm e1 A0 B0 s0/pi1_inj[eqA[eqB e2]] vl. subst.
     exists A. exists m... }
@@ -39,12 +39,12 @@ Proof with eauto.
     apply: conv_trans... }
 Qed.
 
-Lemma sta_sig0_canonical m A B C s :
-  nil ⊢ m : C -> C ≃ Sig0 A B s -> sta_val m ->
+Lemma logical_sig0_canonical m A B C s :
+  nil ⊢ m : C -> C ≃ Sig0 A B s -> logical_val m ->
   exists m1 m2, m = Pair0 m1 m2 s.
 Proof with eauto.
   move e:(nil)=>Γ ty. elim: ty e A B s=>//{Γ m C}.
-  all: try solve[intros; exfalso; (solve_conv||inv_sta_val)].
+  all: try solve[intros; exfalso; (solve_conv||inv_logical_val)].
   { move=>Γ x A wf shs e. subst. inv shs. }
   { move=>Γ A B m n t l tyS _ tym _ tyn _ e1 A0 B0 s0/sig0_inj[eqA[eqB e2]] vl.
     subst. exists m. exists n... }
@@ -53,12 +53,12 @@ Proof with eauto.
     apply: conv_trans... }
 Qed.
 
-Lemma sta_sig1_canonical m A B C s :
-  nil ⊢ m : C -> C ≃ Sig1 A B s -> sta_val m ->
+Lemma logical_sig1_canonical m A B C s :
+  nil ⊢ m : C -> C ≃ Sig1 A B s -> logical_val m ->
   exists m1 m2, m = Pair1 m1 m2 s.
 Proof with eauto.
   move e:(nil)=>Γ ty. elim: ty e A B s=>//{Γ m C}.
-  all: try solve[intros; exfalso; (solve_conv||inv_sta_val)].
+  all: try solve[intros; exfalso; (solve_conv||inv_logical_val)].
   { move=>Γ x A wf shs e. subst. inv shs. }
   { move=>Γ A B m n t l tyS _ tym _ tyn _ e1 A0 B0 s0/sig1_inj[eqA[eqB e2]] vl.
     subst. exists m. exists n... }
@@ -67,11 +67,11 @@ Proof with eauto.
     apply: conv_trans... }
 Qed.
 
-Lemma sta_bool_canonical m C :
-  nil ⊢ m : C -> C ≃ Bool -> sta_val m -> m = TT \/ m = FF.
+Lemma logical_bool_canonical m C :
+  nil ⊢ m : C -> C ≃ Bool -> logical_val m -> m = TT \/ m = FF.
 Proof with eauto.
   move e:(nil)=>Γ ty. elim: ty e=>//{Γ m C}.
-  all: try solve[intros; exfalso; (solve_conv||inv_sta_val)].
+  all: try solve[intros; exfalso; (solve_conv||inv_logical_val)].
   { move=>Γ x A wf shs e. subst. inv shs. }
   { move=>Γ wf e _ vl. left... }
   { move=>Γ wf e _ vl. right... }
@@ -80,12 +80,12 @@ Proof with eauto.
     apply: conv_trans... }
 Qed.
 
-Lemma sta_id_canonical m C A x y :
-  nil ⊢ m : C -> C ≃ Id A x y -> sta_val m ->
+Lemma logical_id_canonical m C A x y :
+  nil ⊢ m : C -> C ≃ Id A x y -> logical_val m ->
   exists n, m = Refl n.
 Proof with eauto.
   move e:(nil)=>Γ ty. elim: ty e A x y=>{Γ m C}.
-  all: try solve[intros; exfalso; (solve_conv||inv_sta_val)].
+  all: try solve[intros; exfalso; (solve_conv||inv_logical_val)].
   { move=>Γ x A wf shs e. subst. inv shs. }
   { move=>Γ A m tym ihm e A0 x y eq vl.
     exists m... }
@@ -94,8 +94,8 @@ Proof with eauto.
     apply: conv_trans... }
 Qed.
 
-Lemma sta_prog m A : nil ⊢ m : A -> (exists n, m ~> n) \/ sta_val m.
-Proof with eauto using sta_step, sta_val.
+Lemma logical_prg m A : nil ⊢ m : A -> (exists n, m ~> n) \/ logical_val m.
+Proof with eauto using logical_step, logical_val.
   move e:(nil)=>Γ ty. elim: ty e=>{Γ m A}.
   { move=>Γ s wf e. right... }
   { move=>Γ x A wf shs e. subst. inv shs. }
@@ -108,14 +108,14 @@ Proof with eauto using sta_step, sta_val.
     { left. exists (App m0 n)... }
     { have[[n0 stn]|vln]:=ihn erefl.
       { left. exists (App m n0)... }
-      { have[A0[n0 e]]:=sta_pi0_canonical tym (convR _ _) vlm. subst.
+      { have[A0[n0 e]]:=logical_pi0_canonical tym (convR _ _) vlm. subst.
         left. exists (n0.[n/])... } } }
   { move=>Γ A B m n s tym ihm tyn ihn e. subst.
     have[[m0 stm]|vlm]:=ihm erefl.
     { left. exists (App m0 n)... }
     { have[[n0 stn]|vln]:=ihn erefl.
       { left. exists (App m n0)... }
-      { have[A0[n0 e]]:=sta_pi1_canonical tym (convR _ _) vlm. subst.
+      { have[A0[n0 e]]:=logical_pi1_canonical tym (convR _ _) vlm. subst.
         left. exists (n0.[n/])... } } }
   { move=>Γ A B s r t l1 l2 leq tyA ihA tyB ihB e. right... }
   { move=>Γ A B s r t l1 l2 leq1 leq2 tyA ihA tyB ihB e. right... }
@@ -132,12 +132,12 @@ Proof with eauto using sta_step, sta_val.
   { move=>Γ A B C m n s t l tyC ihC tym ihm tyn ihn e. subst.
     have[[m' stm]|vlm]:=ihm erefl.
     { left. exists (LetIn C m' n)... }
-    { have[m1[m2 e]]:=sta_sig0_canonical tym (convR _ _) vlm. subst.
+    { have[m1[m2 e]]:=logical_sig0_canonical tym (convR _ _) vlm. subst.
       left. exists n.[m2,m1/]... } }
   { move=>Γ A B C m n s t l tyC ihC tym ihm tyn ihn e. subst.
     have[[m' stm]|vlm]:=ihm erefl.
     { left. exists (LetIn C m' n)... }
-    { have[m1[m2 e]]:=sta_sig1_canonical tym (convR _ _) vlm. subst.
+    { have[m1[m2 e]]:=logical_sig1_canonical tym (convR _ _) vlm. subst.
       left. exists n.[m2,m1/]... } }
   { move=>Γ wf e. right... }
   { move=>Γ wf e. right... }
@@ -145,14 +145,14 @@ Proof with eauto using sta_step, sta_val.
   { move=>Γ A m n1 n2 s l tyA _ tym ihm tyn1 ihn1 tyn2 ihn2 e. subst.
     have[[m' st]|vlm]:=ihm erefl.
     { left. exists (Ifte A m' n1 n2)... }
-    { have[e|e]:=sta_bool_canonical tym (convR _ _) vlm; subst.
+    { have[e|e]:=logical_bool_canonical tym (convR _ _) vlm; subst.
       left. exists n1... left. exists n2... } }
   { move=>Γ A m n s l tyA ihA tym ihm tyn ihn e. right... }
   { move=>Γ A m tym ihm e. right... }
   { move=>Γ A B H P m n s l tyB ihB tyH ihH tyP ihP e. subst.
     have[[P0 stP]|vlP]:=ihP erefl.
     { left. exists (Rw B H P0)... }
-    { have[n0 e]:=sta_id_canonical tyP (convR _ _) vlP. subst.
+    { have[n0 e]:=logical_id_canonical tyP (convR _ _) vlP. subst.
       left. exists H... } }
   { move=>Γ A B m s l eq tym ihm tyB ihB e.
     apply: ihm... }
