coq/theories/logical_unique.v
@@ -1,6 +1,6 @@
 From mathcomp Require Import ssreflect ssrbool eqtype ssrnat seq.
 From Stdlib Require Import ssrfun Classical Utf8.
-Require Export AutosubstSsr ARS sta_inv.
+Require Export AutosubstSsr ARS logical_inv.
 
 Set Implicit Arguments.
 Unset Strict Implicit.
@@ -37,7 +37,7 @@ Inductive head_sim : term -> term -> Prop :=
 | head_sim_refl m : head_sim (Refl m) (Refl m)
 | head_sim_rw A H P : head_sim (Rw A H P) (Rw A H P)
 | head_sim_box : head_sim Box Box
-| head_sim_ptr l : head_sim (Ptr l) (Ptr l).
+| head_sim_heap l : head_sim (Ptr l) (Ptr l).
 
 Inductive sim (m n : term) : Prop :=
 | Sim x y : m ≃ x -> head_sim x y -> y ≃ n -> sim m n.
@@ -90,9 +90,9 @@ Lemma sim_subst x y σ : sim x y -> sim x.[σ] y.[σ].
 Proof with eauto.
   move=>sm. inv sm.
   econstructor.
-  apply: sta_conv_subst...
+  apply: logical_conv_subst...
   apply: head_sim_subst...
-  apply: sta_conv_subst...
+  apply: logical_conv_subst...
 Qed.
 
 Ltac solve_sim :=
@@ -222,7 +222,7 @@ Proof with eauto using sim.
     repeat split... }
 Qed.
 
-Lemma sta_sort_uniq Γ s l1 l2 A :
+Lemma logical_sort_unique Γ s l1 l2 A :
   Γ ⊢ Sort s l1 : A -> sim (Sort U l2) A.
 Proof with eauto using head_sim.
   move e:(Sort s l1)=>n ty. elim: ty s l1 l2 e=>//{Γ n A}.
@@ -233,7 +233,7 @@ Proof with eauto using head_sim.
     apply: sim_transL... }
 Qed.
 
-Lemma sta_has_uniq Γ x A B : sta_has Γ x A -> sta_has Γ x B -> A = B.
+Lemma logical_has_unique Γ x A B : logical_has Γ x A -> logical_has Γ x B -> A = B.
 Proof with eauto.
   move=>hs. elim: hs B=>{Γ x A}.
   { move=>Γ A B hs. inv hs... }
@@ -241,31 +241,31 @@ Proof with eauto.
     rewrite (ih _ H3)... }
 Qed.
 
-Lemma sta_var_uniq Γ A B x :
-  Γ ⊢ Var x : B -> sta_has Γ x A -> sim A B.
+Lemma logical_var_unique Γ A B x :
+  Γ ⊢ Var x : B -> logical_has Γ x A -> sim A B.
 Proof with eauto using sim_reflexive.
   move e:(Var x)=>n ty. elim: ty A x e=>//{Γ n B}.
   { move=>Γ x A wf hs1 A0 x0 [e] hs2; subst.
-    rewrite (sta_has_uniq hs1 hs2)... }
+    rewrite (logical_has_unique hs1 hs2)... }
   { move=>Γ A B m s l eq tym ihm tyB ihB A0 x e hs; subst.
     have eq':=ihm _ _ erefl hs.
     apply: sim_transL... }
 Qed.
 
-Lemma sta_lam0_uniq Γ A B C m s :
+Lemma logical_lam0_unique Γ A B C m s :
   Γ ⊢ Lam0 A m s : C -> (forall C, (A :: Γ) ⊢ m : C -> sim B C) -> sim (Pi0 A B s) C.
 Proof with eauto.
   move e:(Lam0 A m s)=>n ty. elim: ty A B m s e=>//{Γ n C}.
   { move=>Γ A B m s tym ihm A0 B0 m0 s0 [e1 e2 e3] h; subst.
     have eq:=h _ tym. inv eq.
-    econstructor. apply: sta_conv_pi0...
-    constructor... apply: sta_conv_pi0... }
+    econstructor. apply: logical_conv_pi0...
+    constructor... apply: logical_conv_pi0... }
   { move=>Γ A B m s l eq tym ihm tyB ihB A0 B0 m0 s0 e h; subst.
     have eq':=ihm _ _ _ _ erefl h.
     apply: sim_transL... }
 Qed.
 
-Lemma sta_pi0_uniq Γ A B C s l :
+Lemma logical_pi0_unique Γ A B C s l :
   Γ ⊢ Pi0 A B s : C -> sim (Sort s l) C.
 Proof with eauto using head_sim.
   move e:(Pi0 A B s)=>n ty. elim: ty A B s l e=>//{Γ n C}.
@@ -276,7 +276,7 @@ Proof with eauto using head_sim.
     apply: sim_transL... }
 Qed.
 
-Lemma sta_pi1_uniq Γ A B C s l :
+Lemma logical_pi1_unique Γ A B C s l :
   Γ ⊢ Pi1 A B s : C -> sim (Sort s l) C.
 Proof with eauto using head_sim.
   move e:(Pi1 A B s)=>n ty. elim: ty A B s l e=>//{Γ n C}.
@@ -287,20 +287,20 @@ Proof with eauto using head_sim.
     apply: sim_transL... }
 Qed.
 
-Lemma sta_lam1_uniq Γ A B C m s :
+Lemma logical_lam1_unique Γ A B C m s :
   Γ ⊢ Lam1 A m s : C -> (forall C, (A :: Γ) ⊢ m : C -> sim B C) -> sim (Pi1 A B s) C.
 Proof with eauto.
   move e:(Lam1 A m s)=>n ty. elim: ty A B m s e=>//{Γ n C}.
   { move=>Γ A B m s tym ihm A0 B0 m0 s0 [e1 e2 e3] h; subst.
     have eq:=h _ tym. inv eq.
-    econstructor. apply: sta_conv_pi1...
-    constructor... apply: sta_conv_pi1... }
+    econstructor. apply: logical_conv_pi1...
+    constructor... apply: logical_conv_pi1... }
   { move=>Γ A B m s l eq tym ihm tyB ihB A0 B0 m0 s0 e h; subst.
     have eq':=ihm _ _ _ _ erefl h.
     apply: sim_transL... }
 Qed.
 
-Lemma sta_app0_uniq Γ A B C m n s :
+Lemma logical_app0_unique Γ A B C m n s :
   Γ ⊢ App m n : C -> (forall C, Γ ⊢ m : C -> sim (Pi0 A B s) C) -> sim B.[n/] C.
 Proof with eauto.
   move e:(App m n)=>x ty. elim: ty A B m n s e=>//{Γ x C}.
@@ -315,7 +315,7 @@ Proof with eauto.
     apply: sim_transL... }
 Qed.
 
-Lemma sta_app1_uniq Γ A B C m n s :
+Lemma logical_app1_unique Γ A B C m n s :
   Γ ⊢ App m n : C -> (forall C, Γ ⊢ m : C -> sim (Pi1 A B s) C) -> sim B.[n/] C.
 Proof with eauto.
   move e:(App m n)=>x ty. elim: ty A B m n s e=>//{Γ x C}.
@@ -330,7 +330,7 @@ Proof with eauto.
     apply: sim_transL... }
 Qed.
 
-Lemma sta_sig0_uniq Γ A B C s l :
+Lemma logical_sig0_unique Γ A B C s l :
   Γ ⊢ Sig0 A B s : C -> sim (Sort s l) C.
 Proof with eauto using head_sim.
   move e:(Sig0 A B s)=>m ty. elim: ty A B s l e=>//{Γ m C}.
@@ -341,7 +341,7 @@ Proof with eauto using head_sim.
     apply: sim_transL... }
 Qed.
 
-Lemma sta_sig1_uniq Γ A B C s l :
+Lemma logical_sig1_unique Γ A B C s l :
   Γ ⊢ Sig1 A B s : C -> sim (Sort s l) C.
 Proof with eauto using head_sim.
   move e:(Sig1 A B s)=>m ty. elim: ty A B s l e=>//{Γ m C}.
@@ -352,7 +352,7 @@ Proof with eauto using head_sim.
     apply: sim_transL... }
 Qed.
 
-Lemma sta_pair0_uniq Γ A B C m n s :
+Lemma logical_pair0_unique Γ A B C m n s :
   Γ ⊢ Pair0 m n s : C ->
   (forall X Y, Γ ⊢ m : X -> Γ ⊢ n : Y -> sim A X /\ sim B.[m/] Y) ->
   sim (Sig0 A B s) C.
@@ -366,7 +366,7 @@ Proof with eauto.
     apply: sim_transL... }
 Qed.
 
-Lemma sta_pair1_uniq Γ A B C m n s :
+Lemma logical_pair1_unique Γ A B C m n s :
   Γ ⊢ Pair1 m n s : C ->
   (forall X Y, Γ ⊢ m : X -> Γ ⊢ n : Y -> sim A X /\ sim B.[m/] Y) ->
   sim (Sig1 A B s) C.
@@ -380,7 +380,7 @@ Proof with eauto.
     apply: sim_transL... }
 Qed.
 
-Lemma sta_letin_uniq Γ m n A B :
+Lemma logical_letin_unique Γ m n A B :
   Γ ⊢ LetIn A m n : B -> sim A.[m/] B.
 Proof with eauto.
   move e:(LetIn A m n)=>x ty. elim: ty A m n e=>//{Γ B x}.
@@ -393,7 +393,7 @@ Proof with eauto.
     apply: sim_transL... }
 Qed.
 
-Lemma sta_bool_uniq Γ A : Γ ⊢ Bool : A -> sim (Sort U 0) A.
+Lemma logical_bool_unique Γ A : Γ ⊢ Bool : A -> sim (Sort U 0) A.
 Proof with eauto.
   move e:(Bool)=>m ty. elim: ty e=>//{Γ m A}.
   move=>Γ A B m s l eq tym ihm tyB ihB e; subst.
@@ -401,7 +401,7 @@ Proof with eauto.
     apply: sim_transL... }
 Qed.
 
-Lemma sta_tt_uniq Γ A : Γ ⊢ TT : A -> sim Bool A.
+Lemma logical_tt_unique Γ A : Γ ⊢ TT : A -> sim Bool A.
 Proof with eauto.
   move e:(TT)=>m ty. elim: ty e=>//{Γ m A}.
   move=>Γ A B m s l eq tym ihm tyB ihB e; subst.
@@ -409,7 +409,7 @@ Proof with eauto.
     apply: sim_transL... }
 Qed.
 
-Lemma sta_ff_uniq Γ A : Γ ⊢ FF : A -> sim Bool A.
+Lemma logical_ff_unique Γ A : Γ ⊢ FF : A -> sim Bool A.
 Proof with eauto.
   move e:(FF)=>m ty. elim: ty e=>//{Γ m A}.
   move=>Γ A B m s l eq tym ihm tyB ihB e; subst.
@@ -417,7 +417,7 @@ Proof with eauto.
     apply: sim_transL... }
 Qed.
 
-Lemma sta_ifte_uniq Γ m n1 n2 A B :
+Lemma logical_ifte_unique Γ m n1 n2 A B :
   Γ ⊢ Ifte A m n1 n2 : B -> sim A.[m/] B.
 Proof with eauto.
   move e:(Ifte A m n1 n2)=>x ty. elim: ty A m n1 n2 e=>//{Γ B x}.
@@ -429,7 +429,7 @@ Proof with eauto.
     apply: sim_transL... }
 Qed.
 
-Lemma sta_id_uniq Γ A B m n l :
+Lemma logical_id_unique Γ A B m n l :
   Γ ⊢ Id A m n : B -> sim (Sort U l) B.
 Proof with eauto using head_sim.
   move e:(Id A m n)=>x ty. elim: ty A m n l e=>//{Γ x B}.
@@ -440,20 +440,20 @@ Proof with eauto using head_sim.
     apply: sim_transL... }
 Qed.
 
-Lemma sta_refl_uniq Γ A B m :
+Lemma logical_refl_unique Γ A B m :
   Γ ⊢ Refl m : B -> (forall X, Γ ⊢ m : X -> sim A X) -> sim (Id A m m) B.
 Proof with eauto.
   move e:(Refl m)=>x ty. elim: ty m e=>//{Γ x B}.
   { move=>Γ A0 m tym ihm m0[e]h; subst.
     have eq:=h _ tym. inv eq.
-    econstructor. apply: sta_conv_id...
-    constructor... apply: sta_conv_id... }
+    econstructor. apply: logical_conv_id...
+    constructor... apply: logical_conv_id... }
   { move=>Γ A0 B m s l eq tym ihm tyB ihB m0 e h; subst.
     have eq':=ihm _ erefl h.
     apply: sim_transL... }
 Qed.
 
-Lemma sta_rw_uniq Γ A B C H P m n :
+Lemma logical_rw_unique Γ A B C H P m n :
   Γ ⊢ Rw B H P : C -> (forall X, Γ ⊢ P : X -> sim (Id A m n) X) -> sim B.[P,n/] C.
 Proof with eauto.
   move e:(Rw B H P)=>x ty. elim: ty B H P e=>//{Γ x C}.
@@ -461,69 +461,69 @@ Proof with eauto.
     have/sim_id_inj[_[eq1 eq2]]:=h _ tyP.
     have sc:sconv (P .: n .: ids) (P .: n0 .: ids) by move=>[|[|]]//.
     econstructor.
-    apply: sta_conv_compat...
+    apply: logical_conv_compat...
     all: eauto... }
   { move=>Γ A0 B m0 s l eq tym ihm tyB ihB B0 H P e h; subst.
     have eq':=ihm _ _ _ erefl h.
     apply: sim_transL... }
 Qed.
 
-Lemma sta_uniq Γ m A B :
+Lemma logical_unique Γ m A B :
   Γ ⊢ m : A -> Γ ⊢ m : B -> sim A B.
 Proof with eauto.
   move=>ty. elim: ty B=>{Γ m A}.
   { move=>Γ s l B tyB.
-    apply: sta_sort_uniq... }
+    apply: logical_sort_unique... }
   { move=>Γ x A wf hs B ty.
-    apply: sta_var_uniq... }
+    apply: logical_var_unique... }
   { move=>Γ A B s r t l tyA ihA tyB ihB B0 ty.
-    apply: sta_pi0_uniq... }
+    apply: logical_pi0_unique... }
   { move=>Γ A B s r t l tyA ihA tyB ihB B0 ty.
-    apply: sta_pi1_uniq... }
+    apply: logical_pi1_unique... }
   { move=>Γ A B m s tym ihm B0 ty.
-    apply: sta_lam0_uniq... }
+    apply: logical_lam0_unique... }
   { move=>Γ A B m s tym ihm B0 ty.
-    apply: sta_lam1_uniq... }
+    apply: logical_lam1_unique... }
   { move=>Γ A B m n s tym ihm tyn ihn B0 ty.
-    apply: sta_app0_uniq... }
+    apply: logical_app0_unique... }
   { move=>Γ A B m n s tym ihm tyn ihn B0 ty.
-    apply: sta_app1_uniq... }
+    apply: logical_app1_unique... }
   { move=>Γ A B s r t l ord tyA ihA tyB ihB B0 ty.
-    apply: sta_sig0_uniq... }
+    apply: logical_sig0_unique... }
   { move=>Γ A B s r t l ord1 ord2 tyA ihA tyB ihB B0 ty.
-    apply: sta_sig1_uniq... }
+    apply: logical_sig1_unique... }
   { move=>Γ A B m n t l tyS ihS tym ihm tyn ihn B0 ty.
-    apply: sta_pair0_uniq... }
+    apply: logical_pair0_unique... }
   { move=>Γ A B m n t l tyS ihS tym ihm tyn ihn B0 ty.
-    apply: sta_pair1_uniq... }
+    apply: logical_pair1_unique... }
   { move=>Γ A B C m n s t l tyC ihC tym ihm tyn ihn B0 ty.
-    apply: sta_letin_uniq... }
+    apply: logical_letin_unique... }
   { move=>Γ A B C m n s t l tyC ihC tym ihm tyn ihn B0 ty.
-    apply: sta_letin_uniq... }
+    apply: logical_letin_unique... }
   { move=>Γ wf B ty.
-    apply: sta_bool_uniq... }
+    apply: logical_bool_unique... }
   { move=>Γ wf B ty.
-    apply: sta_tt_uniq... }
+    apply: logical_tt_unique... }
   { move=>Γ wf B ty.
-    apply: sta_ff_uniq... }
+    apply: logical_ff_unique... }
   { move=>Γ A m n1 n2 s l tyA ihA tym ihm tyn1 ihn1 tyn2 ihn2 B ty.
-    apply: sta_ifte_uniq... }
+    apply: logical_ifte_unique... }
   { move=>Γ A m n s l tyA ihA tym ihm tyn ihn B ty.
-    apply: sta_id_uniq... }
+    apply: logical_id_unique... }
   { move=>Γ A m tym ihm B ty.
-    apply: sta_refl_uniq... }
+    apply: logical_refl_unique... }
   { move=>Γ A B H P m n s l tyB ihB tyH ihH tyP ihP B0 ty.
-    apply: sta_rw_uniq... }
+    apply: logical_rw_unique... }
   { move=>Γ A B m s l eq tym1 ihm tyB ihB B0 tym2.
     apply: sim_transR.
     apply: ihm...
     apply: conv_sym... }
 Qed.
 
-Theorem sta_unicity Γ m s t l1 l2 :
+Theorem logical_unicity Γ m s t l1 l2 :
   Γ ⊢ m : Sort s l1 -> Γ ⊢ m : Sort t l2 -> s = t.
 Proof.
   move=>tym1 tym2.
   apply: sim_sort.
-  apply: sta_uniq tym1 tym2.
+  apply: logical_unique tym1 tym2.
 Qed.
