coq/theories/program_inv.v
@@ -1,12 +1,12 @@
 From mathcomp Require Import ssreflect ssrbool eqtype ssrnat seq.
 From Stdlib Require Import ssrfun Classical Utf8.
-Require Export AutosubstSsr ARS sta_uniq sta_sr dyn_subst.
+Require Export AutosubstSsr ARS logical_unique logical_sr program_subst.
 
 Set Implicit Arguments.
 Unset Strict Implicit.
 Unset Printing Implicit Defensive.
 
-Lemma dyn_lam0_invX Γ Δ A1 A2 B C m s1 s2 t l :
+Lemma program_lam0_invX Γ Δ A1 A2 B C m s1 s2 t l :
   Γ ; Δ ⊢ Lam0 A1 m s1 : C ->
   C ≃ Pi0 A2 B s2 ->
   (A2 :: Γ) ⊢ B : Sort t l ->
@@ -16,20 +16,20 @@ Proof with eauto.
   elim: tyL A1 A2 B m s1 s2 t l e=>//{Γ Δ C n}.
   { move=>Γ Δ A B m s k tym _ A1 A2 B0 m0
       s1 s2 t l[e1 e2 e3]/pi0_inj[eq1[eq2 e4]]tyB0; subst.
-    have wf:=dyn_type_wf tym. inv wf.
-    have wf:=sta_type_wf tyB0. inv wf.
-    apply: dyn_ctx_conv0.
+    have wf:=program_type_wf tym. inv wf.
+    have wf:=logical_type_wf tyB0. inv wf.
+    apply: program_ctx_conv0.
     apply: conv_sym...
     exact: H4.
-    apply: dyn_conv...
-    apply: sta_ctx_conv... }
+    apply: program_conv...
+    apply: logical_ctx_conv... }
   { move=>Γ Δ A B m s l eq tym ihm tyB A1 A2 B0 m0
       s1 s2 t e eq2 tyB0; subst.
     apply: ihm...
     apply: conv_trans... }
 Qed.
 
-Lemma dyn_lam1_invX Γ Δ A1 A2 B C m s1 s2 t l :
+Lemma program_lam1_invX Γ Δ A1 A2 B C m s1 s2 t l :
   Γ ; Δ ⊢ Lam1 A1 m s1 : C ->
   C ≃ Pi1 A2 B s2 ->
   (A2 :: Γ) ⊢ B : Sort t l ->
@@ -39,41 +39,41 @@ Proof with eauto.
   elim: tyL A1 A2 B m s1 s2 t l e=>//{Γ Δ C n}.
   { move=>Γ Δ A B m s t k tym _ A1 A2 B0 m0
       s1 s2 t0 l[e1 e2 e3]/pi1_inj[eq1[eq2 e4]]tyB0; subst.
-    have wf:=dyn_type_wf tym. inv wf.
-    have wf:=sta_type_wf tyB0. inv wf.
+    have wf:=program_type_wf tym. inv wf.
+    have wf:=logical_type_wf tyB0. inv wf.
     have[A0 rd1 rd2]:=church_rosser eq1.
-    have tyA0t:=sta_rd H4 rd1.
-    have tyA0s:=sta_rd H3 rd2.
-    have e:=sta_unicity tyA0t tyA0s. subst.
+    have tyA0t:=logical_rd H4 rd1.
+    have tyA0s:=logical_rd H3 rd2.
+    have e:=logical_unicity tyA0t tyA0s. subst.
     exists s.
-    apply: dyn_ctx_conv1.
+    apply: program_ctx_conv1.
     apply: conv_sym...
     exact: H3.
-    apply: dyn_conv...
-    apply: sta_ctx_conv... }
+    apply: program_conv...
+    apply: logical_ctx_conv... }
   { move=>Γ Δ A B m s l eq tym ihm tyB A1 A2 B0 m0
       s1 s2 t e eq2 tyB0; subst.
     apply: ihm...
     apply: conv_trans... }
 Qed.
 
-Lemma dyn_lam0_inv Γ Δ m A1 A2 B s1 s2 :
+Lemma program_lam0_inv Γ Δ m A1 A2 B s1 s2 :
   Γ ; Δ ⊢ Lam0 A2 m s2 : Pi0 A1 B s1 -> (A1 :: Γ) ; _: Δ ⊢ m : B.
 Proof with eauto.
   move=>ty.
-  have[t[l/sta_pi0_inv[r[l1[l2[tyB _]]]]]]:=dyn_valid ty.
-  apply: dyn_lam0_invX...
+  have[t[l/logical_pi0_inv[r[l1[l2[tyB _]]]]]]:=program_valid ty.
+  apply: program_lam0_invX...
 Qed.
 
-Lemma dyn_lam1_inv Γ Δ m A1 A2 B s1 s2 :
+Lemma program_lam1_inv Γ Δ m A1 A2 B s1 s2 :
   Γ ; Δ ⊢ Lam1 A2 m s2 : Pi1 A1 B s1 -> exists r, (A1 :: Γ) ; A1 .{r} Δ ⊢ m : B.
 Proof with eauto.
   move=>ty.
-  have[t[l/sta_pi1_inv[r[l1[l2[tyB _]]]]]]:=dyn_valid ty.
-  apply: dyn_lam1_invX...
+  have[t[l/logical_pi1_inv[r[l1[l2[tyB _]]]]]]:=program_valid ty.
+  apply: program_lam1_invX...
 Qed.
 
-Lemma dyn_pair0_invX Γ Δ A B m n s r t l C :
+Lemma program_pair0_invX Γ Δ A B m n s r t l C :
   Γ ; Δ ⊢ Pair0 m n s : C ->
   C ≃ Sig0 A B r ->
   Γ ⊢ Sig0 A B r : Sort t l ->
@@ -83,20 +83,20 @@ Proof with eauto.
   elim: ty A B m n s r t l e=>//{Γ Δ x C}.
   { move=>Γ Δ A B m n t l ty1 tym ihm tyn A0 B0 m0 n0 s r t0 l0[e1 e2 e3]
       /sig0_inj[e4[e5 e6]]ty2; subst.
-    have[s[r0[l1[l2[ord[tyA0[tyB0/sort_inj[e1 e2]]]]]]]]:=sta_sig0_inv ty2. subst.
-    have tym0:Γ ; Δ ⊢ m : A0 by apply: dyn_conv; eauto.
+    have[s[r0[l1[l2[ord[tyA0[tyB0/sort_inj[e1 e2]]]]]]]]:=logical_sig0_inv ty2. subst.
+    have tym0:Γ ; Δ ⊢ m : A0 by apply: program_conv; eauto.
     repeat split...
-    apply: sta_conv.
-    apply: sta_conv_subst.
+    apply: logical_conv.
+    apply: logical_conv_subst.
     all: eauto.
-    apply: sta_esubst...
+    apply: logical_esubst...
     by autosubst. }
   { move=>Γ Δ A B m s l eq tym ihm tyB A0 B0 m0 n s0 r t e eq' ty.
     apply: ihm...
     apply: conv_trans... }
 Qed.
 
-Lemma dyn_pair1_invX Γ Δ A B m n s r t l C :
+Lemma program_pair1_invX Γ Δ A B m n s r t l C :
   Γ ; Δ ⊢ Pair1 m n s : C ->
   C ≃ Sig1 A B r ->
   Γ ⊢ Sig1 A B r : Sort t l ->
@@ -109,35 +109,35 @@ Proof with eauto.
   { move=>Γ Δ1 Δ2 Δ A B m n t l mrg ty1 tym _ tyn _ A0 B0 m0 n0 s r t0 l0
       [e1 e2 e3]/sig1_inj[e4[e5 e6]]ty2; subst.
     exists Δ1. exists Δ2.
-    have[s[r0[l1[l2[ord1[ord2[tyA0[tyB0/sort_inj[e1 e2]]]]]]]]]:=sta_sig1_inv ty2. subst.
-    have tym0:Γ ; Δ1 ⊢ m : A0 by apply: dyn_conv; eauto.
+    have[s[r0[l1[l2[ord1[ord2[tyA0[tyB0/sort_inj[e1 e2]]]]]]]]]:=logical_sig1_inv ty2. subst.
+    have tym0:Γ ; Δ1 ⊢ m : A0 by apply: program_conv; eauto.
     repeat split...
-    apply: dyn_conv.
-    apply: sta_conv_subst.
+    apply: program_conv.
+    apply: logical_conv_subst.
     all: eauto.
-    apply: sta_esubst...
+    apply: logical_esubst...
     by autosubst. }
   { move=>Γ Δ A B m s l eq tym ihm tyB A0 B0 m0 n s0 r t e eq' ty.
     apply: ihm...
     apply: conv_trans... }
 Qed.
 
-Lemma dyn_pair0_inv Γ Δ A B m n s r :
+Lemma program_pair0_inv Γ Δ A B m n s r :
   Γ ; Δ ⊢ Pair0 m n s : Sig0 A B r ->
   s = r /\ Γ ; Δ ⊢ m : A /\ Γ ⊢ n : B.[m/].
 Proof with eauto.
   move=>ty.
-  have[t[l tyS]]:=dyn_valid ty.
-  apply: dyn_pair0_invX...
+  have[t[l tyS]]:=program_valid ty.
+  apply: program_pair0_invX...
 Qed.
 
-Lemma dyn_pair1_inv Γ Δ A B m n s r :
+Lemma program_pair1_inv Γ Δ A B m n s r :
   Γ ; Δ ⊢ Pair1 m n s : Sig1 A B r ->
   exists Δ1 Δ2,
     Δ1 ∘ Δ2 => Δ /\ s = r /\
     Γ ; Δ1 ⊢ m : A /\ Γ ; Δ2 ⊢ n : B.[m/].
 Proof with eauto.
   move=>ty.
-  have[t[l tyS]]:=dyn_valid ty.
-  apply: dyn_pair1_invX...
+  have[t[l tyS]]:=program_valid ty.
+  apply: program_pair1_invX...
 Qed.
