coq/theories/program_sr.v
@@ -1,85 +1,85 @@
 From mathcomp Require Import ssreflect ssrbool eqtype ssrnat seq.
 From Stdlib Require Import ssrfun Classical Utf8.
-Require Export AutosubstSsr ARS sta_sn dyn_inv.
+Require Export AutosubstSsr ARS logical_sn program_inv.
 
 Set Implicit Arguments.
 Unset Strict Implicit.
 Unset Printing Implicit Defensive.
 
-Lemma dyn_sta_step m n A :
+Lemma program_logical_step m n A :
   nil ⊢ m : A -> m ~>> n -> m ~>* n.
-Proof with eauto using sta_step.
+Proof with eauto using logical_step.
   move e:(nil)=>Γ ty. elim: ty e n=>{Γ m A}.
   all: try solve[intros;
                  match goal with
                  | [ H : _ ~>> _ |- _ ] => inv H
                  end].
   { move=>Γ A B m n s tym ihm tyn ihn e n0 st. inv st.
-    { apply: sta_red_app... }
-    { apply: sta_red_app... }
+    { apply: logical_red_app... }
+    { apply: logical_red_app... }
     { apply: star1... }
     { apply: star1... } }
   { move=>Γ A B m n s tym ihm tyn ihn e n0 st. inv st.
-    { apply: sta_red_app... }
-    { apply: sta_red_app... }
+    { apply: logical_red_app... }
+    { apply: logical_red_app... }
     { apply: star1... }
     { apply: star1... } }
   { move=>Γ A B m n t l tyS ihS tym ihm tyn ihn e n0 st. inv st.
-    apply: sta_red_pair0... }
+    apply: logical_red_pair0... }
   { move=>Γ A B m n t l tyS ihS tym ihm tyn ihn e n0 st. inv st.
-    { apply: sta_red_pair1... }
-    { apply: sta_red_pair1... } }
+    { apply: logical_red_pair1... }
+    { apply: logical_red_pair1... } }
   { move=>Γ A B C m n s t l tyC ihC tym ihm tyn ihn e n0 st. inv st.
-    { apply: sta_red_letin... }
+    { apply: logical_red_letin... }
     { apply: star1... }
     { apply: star1... } }
   { move=>Γ A B C m n s t l tyC ihC tym ihm tyn ihn e n0 st. inv st.
-    { apply: sta_red_letin... }
+    { apply: logical_red_letin... }
     { apply: star1... }
     { apply: star1... } }
   { move=>Γ A m n1 n2 s l tyA ihA tym ihm tyn1 ihn1 tyn2 ihn2 e n st. inv st.
-    { apply: sta_red_ifte... }
+    { apply: logical_red_ifte... }
     { apply: star1... }
     { apply: star1... } }
   { move=>Γ A B H P m n s l tyB ihB tyH ihH tyP ihP e n0 st. inv st.
-    have[P0[rdP vlP]]:=sta_vn tyP.
-    have tyP0:=sta_rd tyP rdP.
-    have[n1 e]:=sta_id_canonical tyP0 (convR _ _) vlP. subst.
+    have[P0[rdP vlP]]:=logical_vn tyP.
+    have tyP0:=logical_rd tyP rdP.
+    have[n1 e]:=logical_id_canonical tyP0 (convR _ _) vlP. subst.
     apply: star_trans.
-    apply: sta_red_rw...
+    apply: logical_red_rw...
     apply: star1... }
   { move=>Γ A B m s l eq tym ihm tyB ihB e n st. subst.
     apply: ihm... }
 Qed.
 
-Lemma dyn_sta_red m n A :
+Lemma program_logical_red m n A :
   nil ⊢ m : A -> m ~>>* n -> m ~>* n.
 Proof with eauto.
   move=>ty rd. elim: rd A ty=>{n}...
   move=>m' n rd ih st A tym.
   have rdm:=ih _ tym.
-  have tym':=sta_rd tym rdm.
-  have rdm':=dyn_sta_step tym' st.
+  have tym':=logical_rd tym rdm.
+  have rdm':=program_logical_step tym' st.
   apply: star_trans.
   apply: rdm.
   apply: rdm'.
 Qed.
 
-Lemma dyn_has_type Γ Δ x s A :
-  dyn_has Δ x s A -> dyn_wf Γ Δ -> exists l, Γ ⊢ A : Sort s l.
+Lemma program_has_type Γ Δ x s A :
+  program_has Δ x s A -> program_wf Γ Δ -> exists l, Γ ⊢ A : Sort s l.
 Proof with eauto.
   move=>hs. elim: hs Γ=>{Δ x s A}.
   { move=>Δ A s k Γ wf. inv wf.
-    exists l. apply: sta_eweaken... by asimpl. }
+    exists l. apply: logical_eweaken... by asimpl. }
   { move=>Δ A B x s hs ih Γ wf. inv wf.
     have[lA tyA]:=ih _ H2. 
-    exists lA. apply: sta_eweaken... by asimpl. }
+    exists lA. apply: logical_eweaken... by asimpl. }
   { move=>Δ A x s hs ih Γ wf. inv wf.
     have[lA tyA]:=ih _ H0. 
-    exists lA. apply: sta_eweaken... by asimpl. }
+    exists lA. apply: logical_eweaken... by asimpl. }
 Qed.
 
-Lemma dyn_has_key Δ x s A : dyn_has Δ x s A -> Δ ▷ s.
+Lemma program_has_key Δ x s A : program_has Δ x s A -> Δ ▷ s.
 Proof with eauto using key, key_impure.
   elim=>{Δ x s A}.
   { move=>Δ A [|] k... }
@@ -87,30 +87,30 @@ Proof with eauto using key, key_impure.
   { move=>Δ A x [|] hs k... }
 Qed.
 
-Lemma dyn_val_key Γ Δ m A s l :
-  Γ ; Δ ⊢ m : A -> Γ ⊢ A : Sort s l -> dyn_val m -> Δ ▷ s.
+Lemma program_val_key Γ Δ m A s l :
+  Γ ; Δ ⊢ m : A -> Γ ⊢ A : Sort s l -> program_val m -> Δ ▷ s.
 Proof with eauto using key_impure.
   destruct s...
   move=>ty. elim: ty l=>{Γ Δ m A}.
   { move=>Γ Δ x s A shs dhs wf l0 tyA vl.
-    have[l tyAs]:=dyn_has_type wf shs.
-    have e:=sta_unicity tyA tyAs. subst.
-    apply: dyn_has_key... }
+    have[l tyAs]:=program_has_type wf shs.
+    have e:=logical_unicity tyA tyAs. subst.
+    apply: program_has_key... }
   { move=>Γ Δ A B m s k tym ih l0 tyP vl.
-    have[t[l1[l2[tyB/sort_inj[e1 e2]]]]]:=sta_pi0_inv tyP. by subst. }
+    have[t[l1[l2[tyB/sort_inj[e1 e2]]]]]:=logical_pi0_inv tyP. by subst. }
   { move=>Γ Δ A B m s t k tym ih l0 tyP vl.
-    have[r[l1[l2[tyB/sort_inj[e1 e2]]]]]:=sta_pi1_inv tyP. by subst. }
+    have[r[l1[l2[tyB/sort_inj[e1 e2]]]]]:=logical_pi1_inv tyP. by subst. }
   { move=>Γ Δ A B m n s tym ih tyn l0 tyB vl. inv vl. }
   { move=>Γ Δ1 Δ2 Δ A B m n s mrg tym ihm tyn ihn l0 tyB vl. inv vl. }
   { move=>Γ Δ A B m n t l tyS tym ihm tyn l0 ty vl.
-    have[s[r[l1[l2[ord[tyA[tyB/sort_inj[e1 e2]]]]]]]]:=sta_sig0_inv ty. subst.
+    have[s[r[l1[l2[ord[tyA[tyB/sort_inj[e1 e2]]]]]]]]:=logical_sig0_inv ty. subst.
     inv ord. inv vl... }
   { move=>Γ Δ1 Δ2 Δ A B m n t l mrg tyS tym ihm tyn ihn l0 ty vl.
-    have[s[r[l1[l2[ord1[ord2[tyA[tyB/sort_inj[e1 e2]]]]]]]]]:=sta_sig1_inv ty. subst.
+    have[s[r[l1[l2[ord1[ord2[tyA[tyB/sort_inj[e1 e2]]]]]]]]]:=logical_sig1_inv ty. subst.
     inv ord1. inv ord2. inv vl.
     apply: key_merge...
     apply: ihn...
-    apply: sta_esubst...
+    apply: logical_esubst...
     by autosubst. }
   { move=>Γ Δ1 Δ2 Δ A B C m n s r t l mrg tyC tym ihm tyn ihn l0 ty vl. inv vl. }
   { move=>Γ Δ1 Δ2 Δ A B C m n s r1 r2 t l mrg tyC tym ihm tyn ihn l0 ty vl. inv vl. }
@@ -119,17 +119,17 @@ Proof with eauto using key_impure.
   { move=>Γ Δ1 Δ2 Δ A m n1 n2 s l mrg tyA tym ihm tyn1 ihn1 tyn2 ihn2 l0 ty vl. inv vl. }
   { move=>Γ Δ A B H P m n s l tyB tyH ihH tyP tyB0 l0 vl. inv vl. }
   { move=>Γ Δ A B m s l eq tym ihm tyB1 l0 tyB2 vl.
-    have[r[lA tyA]]:=dyn_valid tym.
+    have[r[lA tyA]]:=program_valid tym.
     have[C rd1 rd2]:=church_rosser eq.
     apply: ihm...
-    have tyCr:=sta_rd tyA rd1.
-    have tyCU:=sta_rd tyB2 rd2.
-    have<-:=sta_unicity tyCr tyCU... }
+    have tyCr:=logical_rd tyA rd1.
+    have tyCU:=logical_rd tyB2 rd2.
+    have<-:=logical_unicity tyCr tyCU... }
 Qed.
 
-Theorem dyn_sr m n A :
+Theorem program_sr m n A :
   nil ; nil ⊢ m : A -> m ~>> n -> nil ; nil ⊢ n : A.
-Proof with eauto using dyn_type, dyn_step, dyn_wf, merge.
+Proof with eauto using program_type, program_step, program_wf, merge.
   move e1:(nil)=>Γ.
   move e2:(nil)=>Δ ty. elim: ty e1 e2 n=>{Γ Δ m A}...
   { move=>Γ Δ x s A wf shs dhs e1 e2 n st. inv st. }
@@ -137,152 +137,152 @@ Proof with eauto using dyn_type, dyn_step, dyn_wf, merge.
   { move=>Γ Δ A B m s t k tym ihm e1 e2 n st. inv st. }
   { move=>Γ Δ A B m n s tym ihm tyn e1 e2 n0 st. inv st.
     { have tym':=ihm erefl erefl _ H2.
-      apply: dyn_app0... }
-    { have tyn':=sta_rd tyn (dyn_sta_step tyn H2).
-      have[t[lP tyP]]:=dyn_valid tym.
-      have[r[l1[l2[tyB _]]]]:=sta_pi0_inv tyP.
-      apply: dyn_conv.
-      apply: sta_conv_beta.
+      apply: program_app0... }
+    { have tyn':=logical_rd tyn (program_logical_step tyn H2).
+      have[t[lP tyP]]:=program_valid tym.
+      have[r[l1[l2[tyB _]]]]:=logical_pi0_inv tyP.
+      apply: program_conv.
+      apply: logical_conv_beta.
       apply: conv_sym.
       apply: star_conv.
-      apply: dyn_sta_step...
-      apply: dyn_app0...
-      have:=sta_subst tyB tyn.
+      apply: program_logical_step...
+      apply: program_app0...
+      have:=logical_subst tyB tyn.
       asimpl... }
-    { have[x[lP tyP]]:=dyn_valid tym.
-      have tym0:=dyn_lam0_inv tym.
-      apply: dyn_subst0... }
+    { have[x[lP tyP]]:=program_valid tym.
+      have tym0:=program_lam0_inv tym.
+      apply: program_subst0... }
     { exfalso.
-      apply: sta_lam1_pi0_false... } }
+      apply: logical_lam1_pi0_false... } }
   { move=>Γ Δ1 Δ2 Δ A B m n s mrg tym ihm tyn ihn e1 e2 n0 st.
     subst. inv mrg. inv st.
     { have tym':=ihm erefl erefl _ H2.
-      apply: dyn_app1... }
+      apply: program_app1... }
     { have tyn':=ihn erefl erefl _ H2.
-      have[x[lP tyP]]:=dyn_valid tym.
-      have[r[l1[l2[tyB _]]]]:=sta_pi1_inv tyP.
-      apply: dyn_conv.
-      apply: sta_conv_beta.
+      have[x[lP tyP]]:=program_valid tym.
+      have[r[l1[l2[tyB _]]]]:=logical_pi1_inv tyP.
+      apply: program_conv.
+      apply: logical_conv_beta.
       apply: conv_sym.
       apply: star_conv.
-      apply: dyn_sta_step...
-      apply: dyn_app1...
-      have:=sta_subst tyB (dyn_sta_type tyn).
+      apply: program_logical_step...
+      apply: program_app1...
+      have:=logical_subst tyB (program_logical_type tyn).
       asimpl... }
     { exfalso.
-      apply: sta_lam0_pi1_false... }
-    { have[x[lP tyP]]:=dyn_valid tym.
-      have[r[l1[l2[tyB _]]]]:=sta_pi1_inv tyP.
-      have[t tym0]:=dyn_lam1_inv tym.
-      have wf:=dyn_type_wf tym0. inv wf.
-      apply: dyn_subst1...
-      apply: (dyn_val_key tyn)... } }
+      apply: logical_lam0_pi1_false... }
+    { have[x[lP tyP]]:=program_valid tym.
+      have[r[l1[l2[tyB _]]]]:=logical_pi1_inv tyP.
+      have[t tym0]:=program_lam1_inv tym.
+      have wf:=program_type_wf tym0. inv wf.
+      apply: program_subst1...
+      apply: (program_val_key tyn)... } }
   { move=>Γ Δ A B m n t l tyS tym ihm tyn e1 e2 n0 st. inv st.
-    have[s[r[l1[l2[ord[tyA[tyB _]]]]]]]:=sta_sig0_inv tyS.
-    apply: dyn_pair0...
-    apply: sta_conv.
-    apply: sta_conv_beta.
+    have[s[r[l1[l2[ord[tyA[tyB _]]]]]]]:=logical_sig0_inv tyS.
+    apply: program_pair0...
+    apply: logical_conv.
+    apply: logical_conv_beta.
     apply: star_conv.
-    apply: (dyn_sta_step (dyn_sta_type tym))...
+    apply: (program_logical_step (program_logical_type tym))...
     apply: tyn.
-    apply: sta_esubst...
+    apply: logical_esubst...
     by autosubst. }
   { move=>Γ Δ1 Δ2 Δ A B m n t l mrg tyS tym ihm tyn ihn e1 e2 n0 st.
     subst. inv mrg. inv st.
-    { have[s[r[l1[l2[ord1[ord2[tyA[tyB _]]]]]]]]:=sta_sig1_inv tyS.
-      apply: dyn_pair1...
-      apply: dyn_conv.
-      apply: sta_conv_beta.
+    { have[s[r[l1[l2[ord1[ord2[tyA[tyB _]]]]]]]]:=logical_sig1_inv tyS.
+      apply: program_pair1...
+      apply: program_conv.
+      apply: logical_conv_beta.
       apply: star_conv.
-      apply: (dyn_sta_step (dyn_sta_type tym))...
+      apply: (program_logical_step (program_logical_type tym))...
       apply: tyn.
-      apply: sta_esubst...
+      apply: logical_esubst...
       by autosubst. }
-    { apply: dyn_pair1... } }
+    { apply: program_pair1... } }
   { move=>Γ Δ1 Δ2 Δ A B C m n s r t l mrg tyC tym ihm tyn ihn e1 e2 n0 st.
     subst. inv mrg. inv st.
-    { apply: dyn_conv.
-      apply: sta_conv_beta.
+    { apply: program_conv.
+      apply: logical_conv_beta.
       apply: conv_sym.
       apply: star_conv.
-      apply: (dyn_sta_step (dyn_sta_type tym))...
-      apply: dyn_letin0...
-      apply: sta_esubst...
+      apply: (program_logical_step (program_logical_type tym))...
+      apply: program_letin0...
+      apply: logical_esubst...
       by autosubst. }
     { inv H3.
-      have[e[tym1 tym2]]:=dyn_pair0_inv tym. subst.
-      have wf:=dyn_type_wf tyn. inv wf. inv H3.
+      have[e[tym1 tym2]]:=program_pair0_inv tym. subst.
+      have wf:=program_type_wf tyn. inv wf. inv H3.
       replace C.[Pair0 m1 m2 t/]
         with C.[Pair0 (Var 1) (Var 0) t .: ren (+2)].[m2,m1/] by autosubst.
-      apply: dyn_substitution...
-      apply: dyn_agree_subst_wk0...
-      apply: dyn_agree_subst_wk1.
-      apply: dyn_val_key tym1 H7 H0.
+      apply: program_substitution...
+      apply: program_agree_subst_wk0...
+      apply: program_agree_subst_wk1.
+      apply: program_val_key tym1 H7 H0.
       apply: merge_sym...
-      apply: dyn_agree_subst_refl...
+      apply: program_agree_subst_refl...
       by autosubst. }
-    { exfalso. apply: sta_pair1_sig0_false... } }
+    { exfalso. apply: logical_pair1_sig0_false... } }
   { move=>Γ Δ1 Δ2 Δ A B C m n s r1 r2 t l mrg tyC tym ihm tyn ihn e1 e2 n0 st.
     subst. inv mrg. inv st.
-    { apply: dyn_conv.
-      apply: sta_conv_beta.
+    { apply: program_conv.
+      apply: logical_conv_beta.
       apply: conv_sym.
       apply: star_conv.
-      apply: (dyn_sta_step (dyn_sta_type tym))...
-      apply: dyn_letin1...
-      apply: sta_esubst...
+      apply: (program_logical_step (program_logical_type tym))...
+      apply: program_letin1...
+      apply: logical_esubst...
       by autosubst. }
-    { exfalso. apply: sta_pair0_sig1_false... }
+    { exfalso. apply: logical_pair0_sig1_false... }
     { inv H3.
-      have[Δ1'[Δ2'[mrg'[e[tym1 tym2]]]]]:=dyn_pair1_inv tym.
-      have wf:=dyn_type_wf tyn. inv wf. inv H3. inv mrg'.
-      have k1:=dyn_val_key tym1 H8 H1.
-      have k2:=dyn_val_key tym2 (sta_subst H6 (dyn_sta_type tym1)) H4.
+      have[Δ1'[Δ2'[mrg'[e[tym1 tym2]]]]]:=program_pair1_inv tym.
+      have wf:=program_type_wf tyn. inv wf. inv H3. inv mrg'.
+      have k1:=program_val_key tym1 H8 H1.
+      have k2:=program_val_key tym2 (logical_subst H6 (program_logical_type tym1)) H4.
       replace C.[Pair1 m1 m2 t/]
         with C.[Pair1 (Var 1) (Var 0) t .: ren (+2)].[m2,m1/] by autosubst.
-      apply: dyn_substitution...
-      apply: dyn_agree_subst_wk1...
-      apply: dyn_agree_subst_wk1...
+      apply: program_substitution...
+      apply: program_agree_subst_wk1...
+      apply: program_agree_subst_wk1...
       by autosubst. } }
   { move=>Γ Δ wf k e1 e2 n st. inv st. }
   { move=>Γ Δ wf k e1 e2 n st. inv st. }
   { move=>Γ Δ1 Δ2 Δ A m n1 n2 s l mrg tyA tym ihm tyn1 ihn1 tyn2 ihn2 e1 e2 n0 st.
     subst. inv mrg. inv st...
-    apply: dyn_conv.
-    apply: sta_conv_beta.
+    apply: program_conv.
+    apply: logical_conv_beta.
     apply: conv_sym.
     apply: star_conv.
-    apply: (dyn_sta_step (dyn_sta_type tym))...
-    apply: dyn_ifte...
-    apply: sta_esubst...
+    apply: (program_logical_step (program_logical_type tym))...
+    apply: program_ifte...
+    apply: logical_esubst...
     by autosubst. }
   { move=>Γ Δ A B H P m n s l tyB tyH ihH tyP e1 e2 n0 st. inv st.
-    have[P0[rdP vlP]]:=sta_vn tyP.
-    have tyP0:=sta_rd tyP rdP.
-    have[m0 e]:=sta_id_canonical tyP0 (convR _ _) vlP. subst.
-    have[r[lI tyI]]:=sta_valid tyP.
-    have[l0[tym[tyn/sort_inj[e1 e2]]]]:=sta_id_inv tyI. subst.
-    have[tym0[eq1 eq2]]:=sta_refl_inv tyP0.
+    have[P0[rdP vlP]]:=logical_vn tyP.
+    have tyP0:=logical_rd tyP rdP.
+    have[m0 e]:=logical_id_canonical tyP0 (convR _ _) vlP. subst.
+    have[r[lI tyI]]:=logical_valid tyP.
+    have[l0[tym[tyn/sort_inj[e1 e2]]]]:=logical_id_inv tyI. subst.
+    have[tym0[eq1 eq2]]:=logical_refl_inv tyP0.
     have sc:sconv (Refl m .: m .: ids) (P .: n .: ids).
     { move=>[|[|]]//=.
-      apply: conv_trans. apply: sta_conv_refl. apply: conv_sym...
+      apply: conv_trans. apply: logical_conv_refl. apply: conv_sym...
       apply: conv_sym. apply: star_conv...
       apply: conv_trans. apply: conv_sym... eauto. }
     have wkB:nil ⊢ B.[P,n/] : Sort s l.
     { replace (Sort s l) with (Sort s l).[P,n/] by eauto.
-      apply: sta_substitution...
+      apply: logical_substitution...
       repeat constructor...
       all: asimpl... }
-    apply: dyn_conv.
-    apply: sta_conv_compat sc.
+    apply: program_conv.
+    apply: logical_conv_compat sc.
     all: eauto. }
 Qed.
 
-Corollary dyn_rd m n A :
+Corollary program_rd m n A :
   nil ; nil ⊢ m : A -> m ~>>* n -> nil ; nil ⊢ n : A.
 Proof with eauto.
   move=>ty rd. elim: rd A ty=>{n}...
   move=>n z rd ih st A tym.
   have tyn:=ih _ tym.
-  apply: dyn_sr...
+  apply: program_sr...
 Qed.
